Refactor terms to be well scoped wrt jump variables
All files have been fixed EXCEPT FOR ANF

CBPV/CK.lean
@@ -6,59 +6,66 @@ open Val Com
 
 namespace CK
 
-inductive F : Type where
-  | app : Val → F
-  | letin : Com → F
-  | fst : F
-  | snd : F
-  | join : Com → F
+inductive F : Nat → Type where
+  | app : Val → F 0
+  | letin {δ} : Com δ → F δ
+  | fst : F 0
+  | snd : F 0
+  | join {δ} : Com δ → F (δ + 1)
 open F
 
-def K := List F
-def CK := Com × K
+inductive K : Nat → Type where
+  | nil : K 0
+  | app {δ} : Val → K δ → K 0
+  | letin {δ} : Com δ → K δ → K 0
+  | fst {δ} : K δ → K 0
+  | snd {δ} : K δ → K 0
+  | join {δ} : Com δ → K δ → K (δ + 1)
+
+def CK := Σ δ, Com δ × K δ
 
 @[simp]
-def renameK (ξ : Nat → Nat) : K → K
-  | [] => []
-  | .app v :: k => app (renameVal ξ v) :: renameK ξ k
-  | .letin m :: k => letin (renameCom (lift ξ) m) :: renameK ξ k
-  | .fst :: k => fst :: renameK ξ k
-  | .snd :: k => snd :: renameK ξ k
-  | .join m :: k => join (renameCom ξ m) :: renameK ξ k
+def K.renameK {δ} (ξ : Nat → Nat) : K δ → K δ
+  | nil => nil
+  | app v k => app (renameVal ξ v) (renameK ξ k)
+  | letin m k => letin (renameCom (lift ξ) m) (renameK ξ k)
+  | fst k => fst (renameK ξ k)
+  | snd k => snd (renameK ξ k)
+  | join m k => join (renameCom ξ m) (renameK ξ k)
 
 @[simp]
-def dismantle (n : Com) : K → Com
-  | [] => n
-  | .app v :: k => dismantle (app n v) k
-  | .letin m :: k => dismantle (letin n m) k
-  | .fst :: k => dismantle (fst n) k
-  | .snd :: k => dismantle (snd n) k
-  | .join m :: k => dismantle (join m n) k
+def dismantle {δ} (n : Com δ) : K δ → Com 0
+  | .nil => n
+  | .app v k => dismantle (app n v) k
+  | .letin m k => dismantle (letin n m) k
+  | .fst k => dismantle (fst n) k
+  | .snd k => dismantle (snd n) k
+  | .join m k => dismantle (join m n) k
 
 section
 set_option hygiene false
 local infix:40 "⤳" => Step
 inductive Step : CK → CK → Prop where
   -- reduction steps
-  | β {m v k} :        ⟨lam m, app v :: k⟩           ⤳ ⟨m⦃v⦄, k⟩
-  | ζ {v m k} :        ⟨ret v, letin m :: k⟩         ⤳ ⟨m⦃v⦄, k⟩
-  | ιl {v m n k} :     ⟨case (inl v) m n, k⟩         ⤳ ⟨m⦃v⦄, k⟩
-  | ιr {v m n k} :     ⟨case (inr v) m n, k⟩         ⤳ ⟨n⦃v⦄, k⟩
-  | π {m k} :          ⟨force (thunk m), k⟩          ⤳ ⟨m, k⟩
-  | π1 {m n k} :       ⟨prod m n, fst :: k⟩          ⤳ ⟨m, k⟩
-  | π2 {m n k} :       ⟨prod m n, snd :: k⟩          ⤳ ⟨n, k⟩
-  | γ {m v k} :        ⟨jump 0 v, join m :: k⟩       ⤳ ⟨m⦃v⦄, k⟩
+  | β {δ m v k} :        ⟨0, lam m, .app v k⟩              ⤳ ⟨δ, weakenJCom δ m⦃v⦄, k⟩
+  | ζ {δ v m k} :        ⟨0, ret v, .letin m k⟩            ⤳ ⟨δ, m⦃v⦄, k⟩
+  | ιl {δ v m n k} :     ⟨δ, case (inl v) m n, k⟩          ⤳ ⟨δ, m⦃v⦄, k⟩
+  | ιr {δ v m n k} :     ⟨δ, case (inr v) m n, k⟩          ⤳ ⟨δ, n⦃v⦄, k⟩
+  | π {δ m k} :          ⟨δ, force (thunk m), k⟩           ⤳ ⟨δ, weakenJCom δ m, k⟩
+  | π1 {δ m n k} :       ⟨0, prod m n, .fst k⟩             ⤳ ⟨δ, weakenJCom δ m, k⟩
+  | π2 {δ m n k} :       ⟨0, prod m n, .snd k⟩             ⤳ ⟨δ, weakenJCom δ n, k⟩
+  | γ {δ m v k} :        ⟨δ + 1, jump 0 v, .join m k⟩      ⤳ ⟨δ, m⦃v⦄, k⟩
   -- congruence rules
-  | app {m v k} :      ⟨app m v, k⟩                  ⤳ ⟨m, app v :: k⟩
-  | letin {m n k} :    ⟨letin m n, k⟩                ⤳ ⟨m, letin n :: k⟩
-  | fst {m k} :        ⟨fst m, k⟩                    ⤳ ⟨m, fst :: k⟩
-  | snd {m k} :        ⟨snd m, k⟩                    ⤳ ⟨m, snd :: k⟩
-  | join {m n k} :     ⟨join m n, k⟩                 ⤳ ⟨n, join m :: k⟩
+  | app {δ m v k} :      ⟨δ, app m v, k⟩                   ⤳ ⟨0, m, .app v k⟩
+  | letin {δ m n k} :    ⟨δ, letin m n, k⟩                 ⤳ ⟨0, m, .letin n k⟩
+  | fst {δ m k} :        ⟨δ, fst m, k⟩                     ⤳ ⟨0, m, .fst k⟩
+  | snd {δ m k} :        ⟨δ, snd m, k⟩                     ⤳ ⟨0, m, .snd k⟩
+  | join {δ m n k} :     ⟨δ, join m n, k⟩                  ⤳ ⟨δ + 1, n, .join m k⟩
   -- drop joins
-  | ret {m v k} :      ⟨ret v, join m :: k⟩          ⤳ ⟨ret v, k⟩
-  | lam {m n k} :      ⟨lam n, join m :: k⟩          ⤳ ⟨lam n, k⟩
-  | prod {m n₁ n₂ k} : ⟨prod n₁ n₂, join m :: k⟩     ⤳ ⟨prod n₁ n₂, k⟩
-  | join't {j m v k} : ⟨jump (j + 1) v, join m :: k⟩ ⤳ ⟨jump j v, k⟩
+  | ret {δ m v k} :      ⟨δ + 1, ret v, .join m k⟩         ⤳ ⟨δ, ret v, k⟩
+  | lam {δ m n k} :      ⟨δ + 1, lam n, .join m k⟩         ⤳ ⟨δ, lam n, k⟩
+  | prod {δ m n₁ n₂ k} : ⟨δ + 1, prod n₁ n₂, .join m k⟩    ⤳ ⟨δ, prod n₁ n₂, k⟩
+  | join't {δ j m v k} : ⟨δ + 1, jump j.succ v, .join m k⟩ ⤳ ⟨δ, jump j v, k⟩
 end
 infix:40 "⤳" => Step
 
@@ -72,21 +79,21 @@ open CK
 section
 set_option hygiene false
 local infix:40 "⇓" => Big
-inductive Big : Com → Com → Prop where
+inductive Big : ∀ {δ}, Com δ → Com δ → Prop where
   -- terminals
   | ret {v} : ret v ⇓ ret v
   | lam {m} : lam m ⇓ lam m
   | prod {m₁ m₂} : prod m₁ m₂ ⇓ prod m₁ m₂
   | jump {j v} : jump j v ⇓ jump j v
   -- eliminators
-  | π {m t} :
-    m ⇓ t →
-    -------------------
+  | π {δ m t} :
+    weakenJCom δ m ⇓ t →
+    --------------------
     force (thunk m) ⇓ t
-  | β {n t m} {v : Val} :
+  | β {δ n t m} {v : Val} :
     n ⇓ lam m →
-    m⦃v⦄ ⇓ t →
-    -----------
+    weakenJCom δ m⦃v⦄ ⇓ t →
+    -----------------------
     app n v ⇓ t
   | ζ {n t v m} :
     n ⇓ ret v →
@@ -101,15 +108,15 @@ inductive Big : Com → Com → Prop where
     m₂⦃v⦄ ⇓ t →
     ----------------------
     case (inr v) m₁ m₂ ⇓ t
-  | π1 {n t m₁ m₂} :
+  | π1 {δ n t m₁ m₂} :
     n ⇓ prod m₁ m₂ →
-    m₁ ⇓ t →
-    ---------
+    weakenJCom δ m₁ ⇓ t →
+    ---------------------
     fst n ⇓ t
-  | π2 {n t m₁ m₂} :
+  | π2 {δ n t m₁ m₂} :
     n ⇓ prod m₁ m₂ →
-    m₂ ⇓ t →
-    ---------
+    weakenJCom δ m₂ ⇓ t →
+    ---------------------
     snd n ⇓ t
   | γ {m n v t} :
     n ⇓ jump 0 v →
@@ -130,7 +137,7 @@ inductive Big : Com → Com → Prop where
     ---------------------
     join m n ⇓ prod n₁ n₂
   | join't {j m n v} :
-    n ⇓ jump (j + 1) v →
+    n ⇓ jump j.succ v →
     -------------------
     join m n ⇓ jump j v
 end
@@ -138,227 +145,218 @@ infix:40 "⇓" => Big
 
 namespace Big
 
-theorem terminal {n} (nfn : nf n) : n ⇓ n := by
+theorem terminal {δ} {n : Com δ} (nfn : nf n) : n ⇓ n := by
   mutual_induction n generalizing nfn
   all_goals simp at nfn <;> constructor
 
-theorem determinism {m t₁ t₂} (r₁ : m ⇓ t₁) (r₂ : m ⇓ t₂) : t₁ = t₂ := by
-  induction r₁ generalizing t₂ <;> cases r₂
+theorem determinism {δ} {m t₁ t₂ : Com δ} (r₁ : m ⇓ t₁) (r₂ : m ⇓ t₂) : t₁ = t₂ := by
+  induction r₁ <;> cases r₂
   case β.β ih₁ ih₂ _ h₁ h₂
-    | ζ.ζ ih₁ ih₂ _ h₁ h₂ =>
-    injection ih₁ h₁ with e; subst e; exact ih₂ h₂
-  case π1.π1 ih₁ ih₂ _ _ h₁ h₂
-    | π2.π2 ih₁ ih₂ _ _ h₁ h₂ =>
-    injection ih₁ h₁ with e₁ e₂; subst e₁ e₂; exact ih₂ h₂
-  case γ.γ ih₁ ih₂ _ h₁ h₂ =>
-    injection ih₁ h₁ with _ e; subst e; exact ih₂ h₂
+    | ζ.ζ ih₁ ih₂ _ h₁ h₂
+    | π1.π1 ih₁ ih₂ _ _ h₁ h₂
+    | π2.π2 ih₁ ih₂ _ _ h₁ h₂
+    | γ.γ ih₁ ih₂ _ h₁ h₂
+    | joinret.joinret ih₁ _ h₁
+    | joinlam.joinlam ih₁ _ h₁
+    | joinprod.joinprod ih₁ _ _ h₁ =>
+    injection ih₁ h₁; subst_vars; first | rfl | simp [ih₂ h₂]
   case γ.joinlam ih _ _ h | γ.joinret ih _ _ h | γ.joinprod ih _ _ _ h
     | joinlam.γ ih _ h _ | joinret.γ ih _ h _ | joinprod.γ ih _ h _
     | γ.join't ih _ _ e h | join't.γ e _ ih _ h _
     | joinret.join't ih _ _ h | join't.joinret ih _ h
     | joinprod.join't ih _ _ h | join't.joinprod ih _ _ h
-    | joinlam.join't ih _ _ h | join't.joinlam ih _ h => cases ih h
+    | joinlam.join't ih _ _ h | join't.joinlam ih _ h
+    | joinret.joinlam ih _ h | joinret.joinprod ih _ _ h
+    | joinlam.joinret ih _ h | joinlam.joinprod ih _ _ h
+    | joinprod.joinret ih _ h | joinprod.joinlam ih _ h => cases ih h
   case join't.join't ih _ _ h =>
-    injection ih h with ej ev; injection ej with ej; subst ej ev; rfl
+    injection ih h with _ ej ev; rw [Fin.succ_inj.mp ej]; simp [ev]
   all_goals apply_rules
-
-theorem app {m n v t} (h : ∀ t, m ⇓ t → n ⇓ t) : app m v ⇓ t → app n v ⇓ t := by
-  intro r; generalize e : Com.app m v = mv at r
-  induction r generalizing m n <;> injection e
-  case β h₁ h₂ _ _ em ev => subst em ev; exact β (h _ h₁) h₂
-
-theorem letin {n₁ n₂ m t} (h : ∀ t, n₁ ⇓ t → n₂ ⇓ t) : letin n₁ m ⇓ t → letin n₂ m ⇓ t := by
-  intro r; generalize e : Com.letin n₁ m = m' at r
-  induction r generalizing m <;> injection e
-  case ζ h₁ h₂ _ _ en em => subst en em; exact ζ (h _ h₁) h₂
-
-theorem fst {m n t} (h : ∀ t, m ⇓ t → n ⇓ t) : fst m ⇓ t → fst n ⇓ t := by
-  intro r; generalize e : Com.fst m = m' at r
-  induction r generalizing m <;> injection e
-  case π1 h₁ h₂ _ _ e => subst e; exact π1 (h _ h₁) h₂
-
-theorem snd {m n t} (h : ∀ t, m ⇓ t → n ⇓ t) : snd m ⇓ t → snd n ⇓ t := by
-  intro r; generalize e : Com.snd m = m' at r
-  induction r generalizing m <;> injection e
-  case π2 h₁ h₂ _ _ e => subst e; exact π2 (h _ h₁) h₂
-
-theorem join {m n₁ n₂ t} (h : ∀ t, n₁ ⇓ t → n₂ ⇓ t) : join m n₁ ⇓ t → join m n₂ ⇓ t := by
-  intro r; generalize e : Com.join m n₁ = m' at r
-  induction r generalizing m <;> injection e
-  case γ h₁ h₂ _ _ em en => subst em en; exact γ (h _ h₁) h₂
-  case join't h₁ _ em en => subst em en; exact join't (h _ h₁)
-  case joinret h₁ _ em en => subst em en; exact joinret (h _ h₁)
-  case joinlam h₁ _ em en => subst em en; exact joinlam (h _ h₁)
-  case joinprod h₁ _ em en => subst em en; exact joinprod (h _ h₁)
 
 end Big
 
 section
 set_option hygiene false
-local infix:40 "≡" => EqVal
-local infix:40 "≡" => EqCom
+local notation:40 m:41 "≡" n:41 => EqVal m n
+local notation:40 m:41 "≡" n:41 => EqCom m n
 mutual
 inductive EqVal : Val → Val → Prop
   | var {x} : var x ≡ var x
   | unit : unit ≡ unit
   | inl {v w : Val} : v ≡ w → inl v ≡ inl w
   | inr {v w : Val} : v ≡ w → inr v ≡ inr w
-  | thunk {m n : Com} : m ≡ n → thunk m ≡ thunk n
+  | thunk {m n : Com 0} : m ≡ n → thunk m ≡ thunk n
   | sym {v w : Val} : w ≡ v → v ≡ w
   | trans {u v w : Val} : u ≡ v → v ≡ w → u ≡ w
 
-inductive EqCom : Com → Com → Prop
+inductive EqCom : ∀ {δ}, Com δ → Com δ → Prop
   -- congruence rules
   | force {v w : Val} : v ≡ w → force v ≡ force w
-  | lam {m n : Com} : m ≡ n → lam m ≡ lam n
-  | app {m n : Com} {v w : Val} : m ≡ n → v ≡ w → app m v ≡ app n w
+  | lam {m n : Com 0} : m ≡ n → lam m ≡ lam n
+  | app {m n : Com 0} {v w : Val} : m ≡ n → v ≡ w → app m v ≡ app n w
   | ret {v w : Val} : v ≡ w → ret v ≡ ret w
-  | letin {n₁ n₂ m₁ m₂ : Com} : m₁ ≡ n₁ → m₂ ≡ n₂ → letin m₁ m₂ ≡ letin n₁ n₂
-  | case {v w : Val} {m₁ n₁ m₂ n₂ : Com} : v ≡ w → m₁ ≡ n₁ → m₂ ≡ n₂ → case v m₁ m₂ ≡ case w n₁ n₂
-  | prod {m₁ m₂ n₁ n₂ : Com} : m₁ ≡ n₁ → m₂ ≡ n₂ → prod m₁ m₂ ≡ prod n₁ n₂
-  | fst {m n : Com} : m ≡ n → fst m ≡ fst n
-  | snd {m n : Com} : m ≡ n → snd m ≡ snd n
-  | join {m₁ m₂ n₁ n₂ : Com} : m₁ ≡ n₁ → m₂ ≡ n₂ → join m₁ m₂ ≡ join n₁ n₂
+  | letin {δ} {m₁ n₁ : Com 0} {m₂ n₂ : Com δ} : m₁ ≡ n₁ → m₂ ≡ n₂ → letin m₁ m₂ ≡ letin n₁ n₂
+  | case {δ} {v w : Val} {m₁ n₁ m₂ n₂ : Com δ} : v ≡ w → m₁ ≡ n₁ → m₂ ≡ n₂ → case v m₁ m₂ ≡ case w n₁ n₂
+  | prod {m₁ m₂ n₁ n₂ : Com 0} : m₁ ≡ n₁ → m₂ ≡ n₂ → prod m₁ m₂ ≡ prod n₁ n₂
+  | fst {m n : Com 0} : m ≡ n → fst m ≡ fst n
+  | snd {m n : Com 0} : m ≡ n → snd m ≡ snd n
+  | join {δ} {m₁ n₁ : Com δ} {m₂ n₂ : Com (δ + 1)} : m₁ ≡ n₁ → m₂ ≡ n₂ → join m₁ m₂ ≡ join n₁ n₂
   | jump {j} {v w : Val} : v ≡ w → jump j v ≡ jump j w
   -- reduction rules
-  | β {m v} : app (lam m) v ≡ m⦃v⦄
+  | β {δ m v} : app (lam m) v ≡ weakenJCom δ m⦃v⦄
   | ζ {m v} : letin (ret v) m ≡ m⦃v⦄
   | ιl {v m₁ m₂} : case (inl v) m₁ m₂ ≡ m₁⦃v⦄
   | ιr {v m₁ m₂} : case (inr v) m₁ m₂ ≡ m₂⦃v⦄
-  | π {m} : force (thunk m) ≡ m
-  | π1 {m₁ m₂} : fst (prod m₁ m₂) ≡ m₁
-  | π2 {m₁ m₂} : snd (prod m₁ m₂) ≡ m₂
+  | π {δ m} : force (thunk m) ≡ weakenJCom δ m
+  | π1 {δ m₁ m₂} : fst (prod m₁ m₂) ≡ weakenJCom δ m₁
+  | π2 {δ m₁ m₂} : snd (prod m₁ m₂) ≡ weakenJCom δ m₂
   | γ {m v} : join m (jump 0 v) ≡ m⦃v⦄
   -- drop joins
   | joinret {m v} : join m (ret v) ≡ ret v
   | joinlam {m n} : join m (lam n) ≡ lam n
   | joinprod {m n₁ n₂} : join m (prod n₁ n₂) ≡ prod n₁ n₂
-  | join't {j m v} : join m (jump (j + 1) v) ≡ jump j v
+  | join't {j m v} : join m (jump j.succ v) ≡ jump j v
   -- partial equivalence
-  | sym {m n : Com} : n ≡ m → m ≡ n
-  | trans {m n p : Com} : m ≡ n → n ≡ p → m ≡ p
+  | sym {δ} {m n : Com δ} : n ≡ m → m ≡ n
+  | trans {δ} {m n p : Com δ} : m ≡ n → n ≡ p → m ≡ p
 end
 end
-infix:40 "≡" => EqVal
-infix:40 "≡" => EqCom
+notation:40 m:41 "≡" n:41 => EqVal m n
+notation:40 m:41 "≡" n:41 => EqCom m n
 
 theorem reflValCom :
   (∀ {v : Val}, v ≡ v) ∧
-  (∀ {m : Com}, m ≡ m) := by
-  refine ⟨λ {v} ↦ ?val, λ {m} ↦ ?com⟩
+  (∀ {δ} {m : Com δ}, m ≡ m) := by
+  refine ⟨λ {v} ↦ ?val, λ {δ m} ↦ ?com⟩
   mutual_induction v, m
   all_goals constructor <;> assumption
 
 @[refl] theorem EqVal.refl : ∀ {v : Val}, v ≡ v := reflValCom.left
-@[refl] theorem EqCom.refl : ∀ {m : Com}, m ≡ m := reflValCom.right
+@[refl] theorem EqCom.refl : ∀ {δ} {m : Com δ}, m ≡ m := reflValCom.right
 
-instance : Trans EqCom EqCom EqCom where
+instance {δ} : Trans (@EqCom δ) (@EqCom δ) (@EqCom δ) where
   trans := .trans
 
 /-* CK machine semantics is sound wrt small-step evaluation semantics *-/
 
-theorem evalCongK {m n k} (r : m ⇒ n) : dismantle m k ⇒ dismantle n k := by
-  induction k generalizing m n
+theorem evalCongK {δ m n} {k : K δ} (r : m ⇒ n) : dismantle m k ⇒ dismantle n k := by
+  induction k
   case nil => simp [r]
-  case cons f _ ih =>
-    cases f
-    all_goals apply ih; constructor; apply r
+  all_goals rename_i ih; apply ih; constructor; apply r
 
-theorem stepEval {m n k₁ k₂} (r : ⟨m, k₁⟩ ⤳ ⟨n, k₂⟩) :
+theorem stepEval {δ₁ δ₂ m n k₁ k₂} (r : ⟨δ₁, m, k₁⟩ ⤳ ⟨δ₂, n, k₂⟩) :
   (dismantle m k₁ ⇒ dismantle n k₂) ∨ (dismantle m k₁ = dismantle n k₂) := by
-  generalize e₁ : (m, k₁) = ck₁ at r
-  generalize e₂ : (n, k₂) = ck₂ at r
+  generalize e₁ : Sigma.mk (β := λ δ ↦ Com δ × K δ) δ₁ (m, k₁) = ck₁ at r
+  generalize e₂ : Sigma.mk (β := λ δ ↦ Com δ × K δ) δ₂ (n, k₂) = ck₂ at r
   induction r generalizing m n k₁ k₂
+  all_goals injection e₁ with eδ e₁; subst eδ
+  all_goals injection e₂ with eδ e₂; subst eδ
   all_goals injection e₁ with em ek₁; subst em ek₁
   all_goals injection e₂ with en ek₂; subst en ek₂
   case app | letin | fst | snd | join => right; rfl
-  all_goals (try simp); left; apply evalCongK; constructor
+  all_goals (try simp); left; apply evalCongK; (try constructor)
+  case β => rw [weakenJSubst]; constructor
 
-theorem stepEvals {m n k₁ k₂} (r : ⟨m, k₁⟩ ⤳⋆ ⟨n, k₂⟩) : dismantle m k₁ ⇒⋆ dismantle n k₂ := by
-  generalize e₁ : (m, k₁) = ck₁ at r
-  generalize e₂ : (n, k₂) = ck₂ at r
-  induction r generalizing m n k₁ k₂
-  case refl => subst e₁; injection e₂ with em ek; subst em ek; rfl
+theorem stepEvals {δ₁ δ₂ m n k₁ k₂} (r : ⟨δ₁, m, k₁⟩ ⤳⋆ ⟨δ₂, n, k₂⟩) : dismantle m k₁ ⇒⋆ dismantle n k₂ := by
+  generalize e₁ : Sigma.mk (β := λ δ ↦ Com δ × K δ) δ₁ (m, k₁) = ck₁ at r
+  generalize e₂ : Sigma.mk (β := λ δ ↦ Com δ × K δ) δ₂ (n, k₂) = ck₂ at r
+  induction r generalizing δ₁ δ₂ m n k₁ k₂
+  case refl =>
+    subst e₁; injection e₂ with eδ emk
+    subst eδ; injection emk with em ek
+    subst em ek; rfl
   case trans ck _ r _ ih =>
     subst e₁ e₂; cases ck; specialize ih rfl rfl
     match stepEval r with
     | .inl r => exact .trans r ih
     | .inr e => simp [e, ih]
 
-theorem stepEvalsNil {m n} : ⟨m, []⟩ ⤳⋆ ⟨n, []⟩ → m ⇒⋆ n := stepEvals
+theorem stepEvalsNil {m n} : ⟨0, m, .nil⟩ ⤳⋆ ⟨0, n, .nil⟩ → m ⇒⋆ n := stepEvals
 
 /-* CK machine semantics is sound wrt big-step semantics *-/
 
-theorem bigCongK {m n t k} (h : ∀ t, n ⇓ t → m ⇓ t) : dismantle n k ⇓ t → dismantle m k ⇓ t := by
-  induction k generalizing m n
+theorem bigCongK {δ m n t} {k : K δ} (h : ∀ t, n ⇓ t → m ⇓ t) : dismantle n k ⇓ t → dismantle m k ⇓ t := by
+  induction k
   case nil => exact h _
-  case cons f _ ih =>
-    cases f <;> refine ih (λ t ↦ ?_)
-    all_goals apply_assumption [Big.app h, Big.letin h, Big.fst h, Big.snd h, Big.join h]
+  all_goals rename_i ih; refine ih (λ t r ↦ ?_)
+  case join => exact join h r
+  all_goals cases r; constructor <;> apply_rules [h]
+  where join {δ n₁ n₂} {m t : Com δ} (h : ∀ t, n₁ ⇓ t → n₂ ⇓ t) : join m n₁ ⇓ t → join m n₂ ⇓ t
+    | .γ h₁ h₂ => .γ (h _ h₁) h₂
+    | .join't h₁ => .join't (h _ h₁)
+    | .joinret h₁ => .joinret (h _ h₁)
+    | .joinlam h₁ => .joinlam (h _ h₁)
+    | .joinprod h₁ => .joinprod (h _ h₁)
 
-theorem bigStep {m n t k₁ k₂} (r : ⟨m, k₁⟩ ⤳ ⟨n, k₂⟩) : dismantle n k₂ ⇓ t → dismantle m k₁ ⇓ t := by
-  generalize em : (m, k₁) = mk at r
-  generalize en : (n, k₂) = nk at r
+theorem bigStep {δ₁ δ₂ m n t k₁ k₂} (r : ⟨δ₁, m, k₁⟩ ⤳ ⟨δ₂, n, k₂⟩) : dismantle n k₂ ⇓ t → dismantle m k₁ ⇓ t := by
+  generalize em : Sigma.mk (β := λ δ ↦ Com δ × K δ) δ₁ (m, k₁) = mk at r
+  generalize en : Sigma.mk (β := λ δ ↦ Com δ × K δ) δ₂ (n, k₂) = nk at r
   induction r generalizing m n k₁ k₂
+  all_goals injection em with eδ em; subst eδ
+  all_goals injection en with eδ em; subst eδ
   all_goals injection em with em ek; subst em ek
-  all_goals injection en with en ek; subst en ek
+  all_goals injection em with en ek; subst en ek
   all_goals apply bigCongK; (try simp) <;> intro t r
-  case β | ζ | π1 | π2 | γ => constructor; constructor; assumption
-  case ιl | ιr | π => constructor; assumption
+  case β | π | π1 | π2 => constructor <;> first | constructor | assumption
+  case ζ | γ | ιl | ιr => constructor <;> first | constructor | assumption
   all_goals cases r
   case ret => exact .joinret .ret
   case lam => exact .joinlam .lam
   case prod => exact .joinprod .prod
   case join't => exact .join't .jump
 
-theorem bigSteps {m n t k₁ k₂} (r : ⟨m, k₁⟩ ⤳⋆ ⟨n, k₂⟩) : dismantle n k₂ ⇓ t → dismantle m k₁ ⇓ t := by
-  generalize em : (m, k₁) = mk at r
-  generalize en : (n, k₂) = nk at r
-  induction r generalizing m n k₁ k₂ <;> intro rn
-  case refl => subst en; injection em with em ek; subst em ek; exact rn
-  case trans rm _ ih => subst en em; exact bigStep rm (ih rfl rfl rn)
+theorem bigSteps {δ₁ δ₂ m n t k₁ k₂} (r : ⟨δ₁, m, k₁⟩ ⤳⋆ ⟨δ₂, n, k₂⟩) : dismantle n k₂ ⇓ t → dismantle m k₁ ⇓ t := by
+  generalize em : Sigma.mk (β := λ δ ↦ Com δ × K δ) δ₁ (m, k₁) = mk at r
+  generalize en : Sigma.mk (β := λ δ ↦ Com δ × K δ) δ₂ (n, k₂) = nk at r
+  induction r generalizing δ₁ δ₂ m n k₁ k₂ <;> intro rn
+  case refl =>
+    subst en; injection em with eδ em
+    subst eδ; injection em with em ek
+    subst em ek; exact rn
+  case trans nk _ rm _ ih =>
+    subst en em; exact bigStep rm (ih rfl rfl rn)
 
-theorem bigStepsNil {m t} (nfn : nf t)  (r : ⟨m, []⟩ ⤳⋆ ⟨t, []⟩) : m ⇓ t :=
+theorem bigStepsNil {m t} (nfn : nf t)  (r : ⟨0, m, .nil⟩ ⤳⋆ ⟨0, t, .nil⟩) : m ⇓ t :=
   bigSteps r (.terminal nfn)
 
 /-* CK machine semantics is complete wrt big-step semantics *-/
 
-theorem stepBig {m n k} (r : m ⇓ n) : ⟨m, k⟩ ⤳⋆ ⟨n, k⟩ := by
-  induction r generalizing k
+theorem stepBig {δ m n k} (r : m ⇓ n) : ⟨δ, m, k⟩ ⤳⋆ ⟨δ, n, k⟩ := by
+  induction r
   case lam | ret | prod | jump => rfl
   case π ih => exact .trans .π ih
   case ιl ih => exact .trans .ιl ih
   case ιr ih => exact .trans .ιr ih
-  case β n t m v _ _ ih₁ ih₂ =>
-    calc ⟨app n v, k⟩
-      _ ⤳  ⟨n, .app v :: k⟩     := .app
-      _ ⤳⋆ ⟨lam m, .app v :: k⟩ := ih₁
-      _ ⤳  ⟨m⦃v⦄, k⟩            := .β
-      _ ⤳⋆ ⟨t, k⟩               := ih₂
-  case ζ n t v m _ _ ih₁ ih₂ =>
-    calc ⟨letin n m, k⟩
-      _ ⤳  ⟨n, .letin m :: k⟩     := .letin
-      _ ⤳⋆ ⟨ret v, .letin m :: k⟩ := ih₁
-      _ ⤳  ⟨m⦃v⦄, k⟩              := .ζ
-      _ ⤳⋆ ⟨t, k⟩                 := ih₂
-  case π1 n t m₁ m₂ _ _ ih₁ ih₂ =>
-    calc ⟨fst n, k⟩
-      _ ⤳  ⟨n, .fst :: k⟩          := .fst
-      _ ⤳⋆ ⟨prod m₁ m₂, .fst :: k⟩ := ih₁
-      _ ⤳  ⟨m₁, k⟩                 := .π1
-      _ ⤳⋆ ⟨t, k⟩                  := ih₂
-  case π2 n t m₁ m₂ _ _ ih₁ ih₂ =>
-    calc ⟨snd n, k⟩
-      _ ⤳  ⟨n, .snd :: k⟩          := .snd
-      _ ⤳⋆ ⟨prod m₁ m₂, .snd :: k⟩ := ih₁
-      _ ⤳  ⟨m₂, k⟩                 := .π2
-      _ ⤳⋆ ⟨t, k⟩                  := ih₂
-  case γ m n v t _ _ ih₁ ih₂ =>
-    calc ⟨join m n, k⟩
-      _ ⤳  ⟨n, .join m :: k⟩        := .join
-      _ ⤳⋆ ⟨jump 0 v, .join m :: k⟩ := ih₁
-      _ ⤳  ⟨m⦃v⦄, k⟩                := .γ
-      _ ⤳⋆ ⟨t, k⟩                   := ih₂
+  case β δ n t m v _ _ ih₁ ih₂ =>
+    calc   ⟨δ, app n v, k⟩
+      _ ⤳  ⟨0, n, .app v k⟩          := .app
+      _ ⤳⋆ ⟨0, lam m, .app v k⟩      := ih₁
+      _ ⤳  ⟨δ, weakenJCom δ m⦃v⦄, k⟩ := .β
+      _ ⤳⋆ ⟨δ, t, k⟩                 := ih₂
+  case ζ δ n t v m _ _ ih₁ ih₂ =>
+    calc   ⟨δ, letin n m, k⟩
+      _ ⤳  ⟨0, n, .letin m k⟩     := .letin
+      _ ⤳⋆ ⟨0, ret v, .letin m k⟩ := ih₁
+      _ ⤳  ⟨δ, m⦃v⦄, k⟩           := .ζ
+      _ ⤳⋆ ⟨δ, t, k⟩              := ih₂
+  case π1 δ n t m₁ m₂ _ _ ih₁ ih₂ =>
+    calc   ⟨δ, fst n, k⟩
+      _ ⤳  ⟨0, n, .fst k⟩          := .fst
+      _ ⤳⋆ ⟨0, prod m₁ m₂, .fst k⟩ := ih₁
+      _ ⤳  ⟨δ, weakenJCom δ m₁, k⟩ := .π1
+      _ ⤳⋆ ⟨δ, t, k⟩               := ih₂
+  case π2 δ n t m₁ m₂ _ _ ih₁ ih₂ =>
+    calc   ⟨δ, snd n, k⟩
+      _ ⤳  ⟨0, n, .snd k⟩          := .snd
+      _ ⤳⋆ ⟨0, prod m₁ m₂, .snd k⟩ := ih₁
+      _ ⤳  ⟨δ, weakenJCom δ m₂, k⟩ := .π2
+      _ ⤳⋆ ⟨δ, t, k⟩               := ih₂
+  case γ δ m n v t _ _ ih₁ ih₂ =>
+    calc   ⟨δ, join m n, k⟩
+      _ ⤳  ⟨δ + 1, n, .join m k⟩        := .join
+      _ ⤳⋆ ⟨δ + 1, jump 0 v, .join m k⟩ := ih₁
+      _ ⤳  ⟨δ, m⦃v⦄, k⟩                 := .γ
+      _ ⤳⋆ ⟨δ, t, k⟩                    := ih₂
   case joinret ih => exact .trans' (.trans .join ih) (.once .ret)
   case joinlam ih => exact .trans' (.trans .join ih) (.once .lam)
   case joinprod ih => exact .trans' (.trans .join ih) (.once .prod)
@@ -366,10 +364,10 @@ theorem stepBig {m n k} (r : m ⇓ n) : ⟨m, k⟩ ⤳⋆ ⟨n, k⟩ := by
 
 /-* CK machine is complete wrt small-step evaluation via big-step *-/
 
-theorem evalBig {m n t} (r : m ⇒ n) : n ⇓ t → m ⇓ t := by
-  induction r generalizing t <;> intro r
+theorem evalBig {δ} {m n t : Com δ} (r : m ⇒ n) : n ⇓ t → m ⇓ t := by
+  induction r <;> intro r
   case π => exact .π r
-  case β => exact .β .lam r
+  case β => rw [← weakenJSubst] at r; exact .β .lam r
   case ζ => exact .ζ .ret r
   case ιl => exact .ιl r
   case ιr => exact .ιr r
@@ -392,38 +390,40 @@ theorem evalBig {m n t} (r : m ⇒ n) : n ⇓ t → m ⇓ t := by
   case prod => cases r; exact .joinprod .prod
   case join't => cases r; exact .join't .jump
 
-theorem evalBigs {m n t} (r : m ⇒⋆ n) : n ⇓ t → m ⇓ t := by
+theorem evalBigs {δ} {m n t : Com δ} (r : m ⇒⋆ n) : n ⇓ t → m ⇓ t := by
   induction r generalizing t <;> intro r
   case refl => exact r
   case trans r' _ ih => exact evalBig r' (ih r)
 
-theorem bigNf {t} (nt : nf t) : t ⇓ t := by
+theorem bigNf {δ t} (nt : @nf δ t) : t ⇓ t := by
   mutual_induction t generalizing nt
   all_goals simp at nt
   all_goals constructor
 
-theorem evalStep {m t} (nt : nf t) (r : m ⇒⋆ t) : ⟨m, []⟩ ⤳⋆ ⟨t, []⟩ :=
+theorem evalStep {m t} (nt : nf t) (r : m ⇒⋆ t) : ⟨0, m, .nil⟩ ⤳⋆ ⟨0, t, .nil⟩ :=
   stepBig (evalBigs r (bigNf nt))
 
 /-* CK machine is sound wrt equational theory *-/
 
-theorem eqCongK {m n : Com} {k} (e : m ≡ n) : dismantle m k ≡ dismantle n k := by
-  induction k generalizing m n
+theorem eqCongK {δ} {m n : Com δ} {k} (e : m ≡ n) : dismantle m k ≡ dismantle n k := by
+  induction k
   case nil => simp [e]
-  case cons f _ ih =>
-    cases f <;> (apply ih; constructor)
-    all_goals first | assumption | rfl
+  all_goals rename_i ih; (apply ih; constructor)
+  all_goals first | assumption | rfl
 
-theorem stepEq {m n k₁ k₂} (r : ⟨m, k₁⟩ ⤳ ⟨n, k₂⟩) : dismantle m k₁ ≡ dismantle n k₂ := by
+theorem stepEq {δ₁ δ₂ m n k₁ k₂} (r : ⟨δ₁, m, k₁⟩ ⤳ ⟨δ₂, n, k₂⟩) : dismantle m k₁ ≡ dismantle n k₂ := by
   cases r
   case app | letin | fst | snd | join => rfl
   all_goals (try simp); apply eqCongK; constructor
 
-theorem stepsEq {m n k₁ k₂} (r : ⟨m, k₁⟩ ⤳⋆ ⟨n, k₂⟩) : dismantle m k₁ ≡ dismantle n k₂ := by
-  generalize e₁ : (m, k₁) = ck₁ at r
-  generalize e₂ : (n, k₂) = ck₂ at r
-  induction r generalizing m n k₁ k₂
-  case refl => subst e₁; injection e₂ with em ek; subst em ek; rfl
+theorem stepsEq {δ₁ δ₂ m n k₁ k₂} (r : ⟨δ₁, m, k₁⟩ ⤳⋆ ⟨δ₂, n, k₂⟩) : dismantle m k₁ ≡ dismantle n k₂ := by
+  generalize e₁ : Sigma.mk (β := λ δ ↦ Com δ × K δ) δ₁ (m, k₁) = ck₁ at r
+  generalize e₂ : Sigma.mk (β := λ δ ↦ Com δ × K δ) δ₂ (n, k₂) = ck₂ at r
+  induction r generalizing δ₁ δ₂ m n k₁ k₂
+  case refl =>
+    subst e₁; injection e₂ with eδ emk
+    subst eδ; injection emk with em ek
+    subst em ek; rfl
   case trans ck _ r _ ih => subst e₁ e₂; exact .trans (stepEq r) (ih rfl rfl)
 
-theorem stepsEqNil {m n} (r : ⟨m, []⟩ ⤳⋆ ⟨n, []⟩) : m ≡ n := stepsEq r
+theorem stepsEqNil {m n} (r : ⟨0, m, .nil⟩ ⤳⋆ ⟨0, n, .nil⟩) : m ≡ n := stepsEq r
