CBPV/Equivalence.lean
@@ -16,7 +16,7 @@ def 𝒱 (A : ValType) (v : Val) (w : Val) : Prop :=
     (∃ v' w', 𝒱 A₂ v' w' ∧ v = inr v' ∧ w = inr w')
   | U B => ∃ m n, ℰ B m n ∧ v = thunk m ∧ w = thunk n
 
-def 𝒞 (B : ComType) (m : Com) (n : Com) : Prop :=
+def 𝒞 {δ} (B : ComType) (m : Com δ) (n : Com δ) : Prop :=
   match B with
   | F A => ∃ v w, 𝒱 A v w ∧ m = ret v ∧ n = ret w
   | Arr A B => ∃ m' n', (∀ v w, 𝒱 A v w → ℰ B (m'⦃v⦄) (n'⦃w⦄)) ∧
@@ -24,7 +24,7 @@ def 𝒞 (B : ComType) (m : Com) (n : Com) : Prop :=
   | .Prod B₁ B₂ => ∃ m₁ m₂ n₁ n₂, ℰ B₁ m₁ n₁ ∧ ℰ B₂ m₂ n₂ ∧
     m = prod m₁ m₂ ∧ n = prod n₁ n₂
 
-def ℰ (B : ComType) (m : Com) (n : Com) :=
+def ℰ {δ} (B : ComType) (m : Com δ) (n : Com δ) :=
   ∃ m' n', m ⇓ₙ m' ∧ n ⇓ₙ n' ∧ 𝒞 B m' n'
 end
 
@@ -34,12 +34,12 @@ notation:40 "(" m:41 "," n:41 ")" "∈" "⟦" B:41 "⟧ᵉ" => ℰ B m n
 
 /-* LE computations are normal and embed into LE evaluations *-/
 
-theorem 𝒞.nf {m n B} (h : (m, n) ∈ ⟦B⟧ᶜ) : nf m ∧ nf n := by
+theorem 𝒞.nf {δ m n B} (h : (m, n) ∈ ⟦B⟧ᶜ) : @nf δ m ∧ @nf δ n := by
   match (generalizing := true) B with
   | F _ | Arr _ _ => unfold 𝒞 at h; let ⟨_, _, _, e₁, e₂⟩ := h; simp [e₁, e₂]
   | .Prod _ _ => unfold 𝒞 at h; let ⟨_, _, _, _, _, _, e₁, e₂⟩ := h; simp [e₁, e₂]
 
-theorem 𝒞ℰ {m n A} (h : 𝒞 A m n) : ℰ A m n := by
+theorem 𝒞ℰ {δ A} {m n : Com δ} (h : 𝒞 A m n) : ℰ A m n := by
   unfold ℰ; let ⟨nfm, nfn⟩ := h.nf; exact ⟨m, n, .refl nfm, .refl nfn, h⟩
 
 /-*-------------------------------
@@ -53,40 +53,40 @@ theorem 𝒱.thunk {m n B} (h : (m, n) ∈ ⟦B⟧ᵉ) : (thunk m, thunk n) ∈ 
 
 namespace ℰ
 
-theorem ret {v w A} (h : (v, w) ∈ ⟦A⟧ᵛ) : (ret v, ret w) ∈ ⟦F A⟧ᵉ := by
+theorem ret {δ v w A} (h : (v, w) ∈ ⟦A⟧ᵛ) : (@ret δ v, @ret δ w) ∈ ⟦F A⟧ᵉ := by
   apply 𝒞ℰ; simp [ℰ, 𝒞, h]
 
-theorem lam {m n A B} (h : ∀ v w, (v, w) ∈ ⟦A⟧ᵛ → (m⦃v⦄, n⦃w⦄) ∈ ⟦B⟧ᵉ) : (lam m, lam n) ∈ ⟦Arr A B⟧ᵉ := by
+theorem lam {δ m n A B} (h : ∀ v w, (v, w) ∈ ⟦A⟧ᵛ → (m⦃v⦄, n⦃w⦄) ∈ ⟦B⟧ᵉ) : (@lam δ m, @lam δ n) ∈ ⟦Arr A B⟧ᵉ := by
   apply 𝒞ℰ; simp [ℰ, 𝒞] at *; exact h
 
-theorem prod {m₁ m₂ n₁ n₂ B₁ B₂} (hB₁ : (m₁, n₁) ∈ ⟦B₁⟧ᵉ) (hB₂ : (m₂, n₂) ∈ ⟦B₂⟧ᵉ) : (prod m₁ m₂, prod n₁ n₂) ∈ ⟦Prod B₁ B₂⟧ᵉ:= by
+theorem prod {δ m₁ m₂ n₁ n₂ B₁ B₂} (hB₁ : (m₁, n₁) ∈ ⟦B₁⟧ᵉ) (hB₂ : (m₂, n₂) ∈ ⟦B₂⟧ᵉ) : (@prod δ m₁ m₂, @prod δ n₁ n₂) ∈ ⟦Prod B₁ B₂⟧ᵉ:= by
   apply 𝒞ℰ; unfold 𝒞; exact ⟨_, _, _, _, hB₁, hB₂, rfl, rfl⟩
 
 /-*-----------------------
   Inversion lemmas on LE
 -----------------------*-/
 
-theorem ret_inv {m n A} (h : (m, n) ∈ ⟦F A⟧ᵉ) : ∃ v w, m ⇒⋆ .ret v ∧ n ⇒⋆ .ret w ∧ (v, w) ∈ ⟦A⟧ᵛ := by
+theorem ret_inv {δ m n A} (h : (m, n) ∈ ⟦F A⟧ᵉ) : ∃ v w, m ⇒⋆ @Com.ret δ v ∧ n ⇒⋆ @Com.ret δ w ∧ (v, w) ∈ ⟦A⟧ᵛ := by
   unfold ℰ 𝒞 at h
   let ⟨_, _, ⟨r₁, _⟩, ⟨r₂, _⟩, _, _, h, e₁, e₂⟩ := h
   subst e₁ e₂; exact ⟨_, _, r₁, r₂, h⟩
 
-theorem lam_inv {m₁ m₂ A B} (h : (m₁, m₂) ∈ ⟦Arr A B⟧ᵉ) : ∃ n₁ n₂, m₁ ⇒⋆ .lam n₁ ∧ m₂ ⇒⋆ .lam n₂ ∧ (∀ v w, (v, w) ∈ ⟦A⟧ᵛ → (n₁⦃v⦄, n₂⦃w⦄) ∈ ⟦B⟧ᵉ) := by
+theorem lam_inv {δ m₁ m₂ A B} (h : (m₁, m₂) ∈ ⟦Arr A B⟧ᵉ) : ∃ n₁ n₂, m₁ ⇒⋆ @Com.lam δ n₁ ∧ m₂ ⇒⋆ @Com.lam δ n₂ ∧ (∀ v w, (v, w) ∈ ⟦A⟧ᵛ → (n₁⦃v⦄, n₂⦃w⦄) ∈ ⟦B⟧ᵉ) := by
   unfold ℰ 𝒞 at h
   let ⟨_, _, ⟨r₁, _⟩, ⟨r₂, _⟩, _, _, h, e₁, e₂⟩ := h
   subst e₁ e₂; exact ⟨_, _, r₁, r₂, h⟩
 
-theorem prod_inv {m n B₁ B₂} (h : (m, n) ∈ ⟦Prod B₁ B₂⟧ᵉ) : ∃ m₁ m₂ n₁ n₂, m ⇒⋆ .prod m₁ m₂ ∧ n ⇒⋆ .prod n₁ n₂ ∧ (m₁, n₁) ∈ ⟦B₁⟧ᵉ ∧ (m₂, n₂) ∈ ⟦B₂⟧ᵉ := by
+theorem prod_inv {δ m n B₁ B₂} (h : (m, n) ∈ ⟦Prod B₁ B₂⟧ᵉ) : ∃ m₁ m₂ n₁ n₂, m ⇒⋆ @Com.prod δ m₁ m₂ ∧ n ⇒⋆ @Com.prod δ n₁ n₂ ∧ (m₁, n₁) ∈ ⟦B₁⟧ᵉ ∧ (m₂, n₂) ∈ ⟦B₂⟧ᵉ := by
   unfold ℰ 𝒞 at h
   let ⟨_, _, ⟨r₁, _⟩, ⟨r₂, _⟩, _, _, _, _, h₁, h₂, e₁, e₂⟩ := h
   subst e₁ e₂; exact ⟨_, _, _, _, r₁, r₂, h₁, h₂⟩
 
-theorem fst {m n B₁ B₂} (h : (m, n) ∈ ⟦Prod B₁ B₂⟧ᵉ) : ∃ m₁ m₂ n₁ n₂, m ⇒⋆ .prod m₁ m₂ ∧ n ⇒⋆ .prod n₁ n₂ ∧ (m₁, n₁) ∈ ⟦B₁⟧ᵉ := by
+theorem fst {δ m n B₁ B₂} (h : (m, n) ∈ ⟦Prod B₁ B₂⟧ᵉ) : ∃ m₁ m₂ n₁ n₂, m ⇒⋆ @Com.prod δ m₁ m₂ ∧ n ⇒⋆ @Com.prod δ n₁ n₂ ∧ (m₁, n₁) ∈ ⟦B₁⟧ᵉ := by
   unfold ℰ 𝒞 at h
   let ⟨_, _, ⟨r₁, _⟩, ⟨r₂, _⟩, _, _, _, _, h, _, e₁, e₂⟩ := h
   subst e₁ e₂; exact ⟨_, _, _, _, r₁, r₂, h⟩
 
-theorem snd {m n B₁ B₂} (h : (m, n) ∈ ⟦Prod B₁ B₂⟧ᵉ) : ∃ m₁ m₂ n₁ n₂, m ⇒⋆ .prod m₁ m₂ ∧ n ⇒⋆ .prod n₁ n₂ ∧ (m₂, n₂) ∈ ⟦B₂⟧ᵉ := by
+theorem snd {δ m n B₁ B₂} (h : (m, n) ∈ ⟦Prod B₁ B₂⟧ᵉ) : ∃ m₁ m₂ n₁ n₂, m ⇒⋆ @Com.prod δ m₁ m₂ ∧ n ⇒⋆ @Com.prod δ n₁ n₂ ∧ (m₂, n₂) ∈ ⟦B₂⟧ᵉ := by
   unfold ℰ 𝒞 at h
   let ⟨_, _, ⟨r₁, _⟩, ⟨r₂, _⟩, _, _, _, _, _, h, e₁, e₂⟩ := h
   subst e₁ e₂; exact ⟨_, _, _, _, r₁, r₂, h⟩
@@ -97,17 +97,17 @@ end ℰ
   LE is a PER
 ------------*-/
 
-theorem sym𝒞ℰ {B} (𝒞sym : ∀ {m n}, (m, n) ∈ ⟦B⟧ᶜ → (n, m) ∈ ⟦B⟧ᶜ) :
-  ∀ {m n}, (m, n) ∈ ⟦B⟧ᵉ → (n, m) ∈ ⟦B⟧ᵉ := by
-  intro _ _ h
+theorem sym𝒞ℰ {B} (𝒞sym : ∀ {δ} {m n : Com δ}, (m, n) ∈ ⟦B⟧ᶜ → (n, m) ∈ ⟦B⟧ᶜ) :
+  ∀ {δ} {m n : Com δ}, (m, n) ∈ ⟦B⟧ᵉ → (n, m) ∈ ⟦B⟧ᵉ := by
+  intro _ _ _ h
   unfold ℰ at *
   let ⟨_, _, nm, nn, hB⟩ := h
   exact ⟨_, _, nn, nm, 𝒞sym hB⟩
 
 theorem sym𝒱𝒞 :
-  (∀ {v w A}, (v, w) ∈ ⟦A⟧ᵛ → (w, v) ∈ ⟦A⟧ᵛ) ∧
-  (∀ {m n B}, (m, n) ∈ ⟦B⟧ᶜ → (n, m) ∈ ⟦B⟧ᶜ) := by
-  refine ⟨λ {v w A} h ↦ ?val, λ {m n B} h ↦ ?com⟩
+  (∀ {A v w}, (v, w) ∈ ⟦A⟧ᵛ → (w, v) ∈ ⟦A⟧ᵛ) ∧
+  (∀ {δ B} {m n : Com δ}, (m, n) ∈ ⟦B⟧ᶜ → (n, m) ∈ ⟦B⟧ᶜ) := by
+  refine ⟨λ {A v w} h ↦ ?val, λ {δ B m n} h ↦ ?com⟩
   mutual_induction A, B
   case Unit => unfold 𝒱 at *; simp [h]
   case Sum ihA₁ ihA₂ =>
@@ -136,9 +136,9 @@ def 𝒱.sym := @sym𝒱𝒞.left
 def 𝒞.sym := @sym𝒱𝒞.right
 def ℰ.sym {B} := @sym𝒞ℰ B 𝒞.sym
 
-theorem trans𝒞ℰ {B} (𝒞trans : ∀ {m₁ m₂ m₃}, (m₁, m₂) ∈ ⟦B⟧ᶜ → (m₂, m₃) ∈ ⟦B⟧ᶜ → (m₁, m₃) ∈ ⟦B⟧ᶜ) :
-  ∀ {m₁ m₂ m₃}, (m₁, m₂) ∈ ⟦B⟧ᵉ → (m₂, m₃) ∈ ⟦B⟧ᵉ → (m₁, m₃) ∈ ⟦B⟧ᵉ := by
-  intro _ _ _ h₁₂ h₂₃
+theorem trans𝒞ℰ {B} (𝒞trans : ∀ {δ} {m₁ m₂ m₃ : Com δ}, (m₁, m₂) ∈ ⟦B⟧ᶜ → (m₂, m₃) ∈ ⟦B⟧ᶜ → (m₁, m₃) ∈ ⟦B⟧ᶜ) :
+  ∀ {δ} {m₁ m₂ m₃ : Com δ}, (m₁, m₂) ∈ ⟦B⟧ᵉ → (m₂, m₃) ∈ ⟦B⟧ᵉ → (m₁, m₃) ∈ ⟦B⟧ᵉ := by
+  intro _ _ _ _ h₁₂ h₂₃
   unfold ℰ at *
   let ⟨m, m', nm, nm', hB₁₂⟩ := h₁₂
   let ⟨n', n, nn', nn, hB₂₃⟩ := h₂₃
@@ -146,9 +146,9 @@ theorem trans𝒞ℰ {B} (𝒞trans : ∀ {m₁ m₂ m₃}, (m₁, m₂) ∈ ⟦
   exact ⟨m, n, nm, nn, 𝒞trans hB₁₂ hB₂₃⟩
 
 theorem trans𝒱𝒞 :
-  (∀ {v₁ v₂ v₃ A}, (v₁, v₂) ∈ ⟦A⟧ᵛ → (v₂, v₃) ∈ ⟦A⟧ᵛ → (v₁, v₃) ∈ ⟦A⟧ᵛ) ∧
-  (∀ {m₁ m₂ m₃ B}, (m₁, m₂) ∈ ⟦B⟧ᶜ → (m₂, m₃) ∈ ⟦B⟧ᶜ → (m₁, m₃) ∈ ⟦B⟧ᶜ) := by
-  refine ⟨λ {v₁ v₂ v₃ A} h₁₂ h₂₃ ↦ ?val, λ {m₁ m₂ m₃ B} h₁₂ h₂₃ ↦ ?com⟩
+  (∀ {A v₁ v₂ v₃}, (v₁, v₂) ∈ ⟦A⟧ᵛ → (v₂, v₃) ∈ ⟦A⟧ᵛ → (v₁, v₃) ∈ ⟦A⟧ᵛ) ∧
+  (∀ {δ B} {m₁ m₂ m₃ : Com δ}, (m₁, m₂) ∈ ⟦B⟧ᶜ → (m₂, m₃) ∈ ⟦B⟧ᶜ → (m₁, m₃) ∈ ⟦B⟧ᶜ) := by
+  refine ⟨λ {A v₁ v₂ v₃} h₁₂ h₂₃ ↦ ?val, λ {δ B m₁ m₂ m₃} h₁₂ h₂₃ ↦ ?com⟩
   mutual_induction A, B
   case Unit =>
     unfold 𝒱 at *
@@ -176,20 +176,20 @@ theorem trans𝒱𝒞 :
     unfold 𝒞 at *
     let ⟨_, _, hA₁₂, el₁, el₂⟩ := h₁₂
     let ⟨_, _, hA₂₃, er₂, er₃⟩ := h₂₃
-    subst el₁ el₂ er₃; injection er₂ with e; subst e
+    subst el₁ el₂ er₃; injection er₂ with _ e; subst e
     exact ⟨_, _, ih hA₁₂ hA₂₃, rfl, rfl⟩
   case Arr ihA ihB =>
     unfold 𝒞; unfold 𝒞 at h₁₂ h₂₃
     let ⟨m, m', hB₁₂, el₁, el₂⟩ := h₁₂
     let ⟨_, n, hB₂₃, er₂, er₃⟩ := h₂₃
-    subst el₁ el₂ er₃; injection er₂ with e; subst e
+    subst el₁ el₂ er₃; injection er₂ with _ e; subst e
     refine ⟨_, _, λ v w hA ↦ ?_, rfl, rfl⟩
     apply trans𝒞ℰ ihB (hB₁₂ v w hA) (hB₂₃ w w (ihA hA.sym hA))
   case Prod ihB₁ ihB₂ =>
     unfold 𝒞; unfold 𝒞 at h₁₂ h₂₃
     let ⟨_, _, _, _, hA₁₁, hA₁₂, el₁, el₂⟩ := h₁₂
     let ⟨_, _, _, _, hA₂₁, hA₂₂, er₁, er₂⟩ := h₂₃
-    subst el₁ el₂ er₂; injection er₁ with e₁ e₂; subst e₁ e₂
+    subst el₁ el₂ er₂; injection er₁ with _ e₁ e₂; subst e₁ e₂
     refine ⟨_, _, _, _, trans𝒞ℰ ihB₁ hA₁₁ hA₂₁, trans𝒞ℰ ihB₂ hA₁₂ hA₂₂, rfl, rfl⟩
 
 def 𝒱.trans := @trans𝒱𝒞.left
@@ -202,18 +202,29 @@ def ℰ.trans {B} := @trans𝒞ℰ B 𝒞.trans
 
 namespace ℰ
 
-theorem bwds {m m' n n' B} (rm : m ⇒⋆ m') (rn : n ⇒⋆ n') (h : (m', n') ∈ ⟦B⟧ᵉ) : (m, n) ∈ ⟦B⟧ᵉ := by
+theorem bwds {δ B} {m m' n n' : Com δ} (rm : m ⇒⋆ m') (rn : n ⇒⋆ n') (h : (m', n') ∈ ⟦B⟧ᵉ) : (m, n) ∈ ⟦B⟧ᵉ := by
   unfold ℰ at *
   let ⟨m'', n'', nm', nn', h⟩ := h
   exact ⟨m'', n'', nm'.bwds rm, nn'.bwds rn, h⟩
 
-theorem bwdsRejoin {m m' n n' js₁ js₂ B} (rm : m ⇒⋆ m') (rn : n ⇒⋆ n') (h : (m', n') ∈ ⟦B⟧ᵉ) : (rejoin m js₁, rejoin n js₂) ∈ ⟦B⟧ᵉ := by
+theorem bwdsRejoin {δ B js₁ js₂} {m m' n n' : Com 0} (rm : m ⇒⋆ m') (rn : n ⇒⋆ n') (h : (m', n') ∈ ⟦B⟧ᵉ) :
+  (rejoin (weakenJCom δ m) js₁, rejoin (weakenJCom δ n) js₂) ∈ ⟦B⟧ᵉ := by
   unfold ℰ at *
   let ⟨m'', n'', nm', nn', h⟩ := h
   refine ⟨m'', n'', nm'.bwdsRejoin rm, nn'.bwdsRejoin rn, h⟩
 
-theorem bwd {m m' n n' B} (rm : m ⇒ m') (rn : n ⇒ n') : (m', n') ∈ ⟦B⟧ᵉ → (m, n) ∈ ⟦B⟧ᵉ := ℰ.bwds (.once rm) (.once rn)
-theorem bwdRejoin {m m' n n' js₁ js₂ B} (rm : m ⇒ m') (rn : n ⇒ n') : (m', n') ∈ ⟦B⟧ᵉ → (rejoin m js₁, rejoin n js₂) ∈ ⟦B⟧ᵉ := ℰ.bwdsRejoin (.once rm) (.once rn)
+theorem bwdsRejoin0 {δ B js₁ js₂} {m m' n n' : Com 0} (rm : m ⇒⋆ weakenJCom 0 m') (rn : n ⇒⋆ weakenJCom 0 n') (h : (m', n') ∈ ⟦B⟧ᵉ) :
+  (rejoin (weakenJCom δ m) js₁, rejoin (weakenJCom δ n) js₂) ∈ ⟦B⟧ᵉ := by
+  rw [weakenJCom0] at rm rn; exact bwdsRejoin rm rn h
+
+theorem bwd {δ B} {m m' n n' : Com δ} (rm : m ⇒ m') (rn : n ⇒ n') :
+  (m', n') ∈ ⟦B⟧ᵉ → (m, n) ∈ ⟦B⟧ᵉ := ℰ.bwds (.once rm) (.once rn)
+theorem bwdRejoin {δ B js₁ js₂} {m m' n n' : Com 0} (rm : m ⇒ m') (rn : n ⇒ n') :
+  (m', n') ∈ ⟦B⟧ᵉ → (rejoin (weakenJCom δ m) js₁, rejoin (weakenJCom δ n) js₂) ∈ ⟦B⟧ᵉ :=
+  ℰ.bwdsRejoin (.once rm) (.once rn)
+theorem bwdRejoin0 {δ B js₁ js₂} {m m' n n' : Com 0} (rm : m ⇒ weakenJCom 0 m') (rn : n ⇒ weakenJCom 0 n') :
+  (m', n') ∈ ⟦B⟧ᵉ → (rejoin (weakenJCom δ m) js₁, rejoin (weakenJCom δ n) js₂) ∈ ⟦B⟧ᵉ :=
+  ℰ.bwdsRejoin0 (.once rm) (.once rn)
 
 end ℰ
 
@@ -244,21 +255,21 @@ end semCtxt
 section
 set_option hygiene false
 local notation:40 Δ:41 "⊨" js₁:41 "~" js₂:41 => semDtxt Δ js₁ js₂
-inductive semDtxt : Dtxt → J → J → Prop where
+inductive semDtxt : ∀ {δ}, Dtxt δ → J δ → J δ → Prop where
   | nil : ⬝ ⊨ .nil ~ .nil
-  | cons {Δ : Dtxt} {js₁ js₂ m n A B} : Δ ⊨ js₁ ~ js₂ →
+  | cons {δ} {Δ : Dtxt δ} {js₁ js₂ m n A B} : Δ ⊨ js₁ ~ js₂ →
     (∀ {v w}, (v, w) ∈ ⟦ A ⟧ᵛ → (rejoin (m⦃v⦄) js₁, rejoin (n⦃w⦄) js₂) ∈ ⟦ B ⟧ᵉ) →
     Δ ∷ A ↗ B ⊨ .cons m js₁ ~ .cons n js₂
 end
 notation:40 Δ:41 "⊨" js₁:41 "~" js₂:41 => semDtxt Δ js₁ js₂
 
-theorem semDtxt.sym {Δ : Dtxt} {js₁ js₂} (h : Δ ⊨ js₁ ~ js₂) : Δ ⊨ js₂ ~ js₁ := by
+theorem semDtxt.sym {δ} {Δ : Dtxt δ} {js₁ js₂} (h : Δ ⊨ js₁ ~ js₂) : Δ ⊨ js₂ ~ js₁ := by
   induction h
   case nil => exact .nil
   case cons h ih => exact .cons ih (λ hvw ↦  .sym (h hvw.sym))
 
-theorem semDtxt.trans {Δ : Dtxt} {js₁ js₂ js₃} (h₁₂ : Δ ⊨ js₁ ~ js₂) (h₂₃ : Δ ⊨ js₂ ~ js₃) : Δ ⊨ js₁ ~ js₃ := by
-  induction h₁₂ generalizing js₃
+theorem semDtxt.trans {δ} {Δ : Dtxt δ} {js₁ js₂ js₃} (h₁₂ : Δ ⊨ js₁ ~ js₂) (h₂₃ : Δ ⊨ js₂ ~ js₃) : Δ ⊨ js₁ ~ js₃ := by
+  induction h₁₂
   case nil => exact h₂₃
   case cons h₁₂ ih =>
     cases h₂₃; case cons hjs h₂₃ =>
@@ -268,7 +279,7 @@ theorem semDtxt.trans {Δ : Dtxt} {js₁ js₂ js₃} (h₁₂ : Δ ⊨ js₁ ~ 
 /-* Semantic equivalence of values and computations *-/
 
 @[simp] def semVal (Γ : Ctxt) (v w : Val) A := ∀ {σ τ}, Γ ⊨ σ ~ τ → (v⦃σ⦄, w⦃τ⦄) ∈ ⟦ A ⟧ᵛ
-@[simp] def semCom (Γ : Ctxt) (Δ : Dtxt) (m n : Com) B := ∀ {σ τ}, Γ ⊨ σ ~ τ → ∀ {js₁ js₂}, Δ ⊨ js₁ ~ js₂ → (rejoin (m⦃σ⦄) js₁, rejoin (n⦃τ⦄) js₂) ∈ ⟦ B ⟧ᵉ
+@[simp] def semCom (Γ : Ctxt) {δ} (Δ : Dtxt δ) (m n : Com δ) B := ∀ {σ τ}, Γ ⊨ σ ~ τ → ∀ {js₁ js₂}, Δ ⊨ js₁ ~ js₂ → (rejoin (m⦃σ⦄) js₁, rejoin (n⦃τ⦄) js₂) ∈ ⟦ B ⟧ᵉ
 notation:40 Γ:41 "⊨" v:41 "~" w:41 "∶" A:41 => semVal Γ v w A
 notation:40 Γ:41 "∣" Δ:41 "⊨" m:41 "~" n:41 "∶" B:41 => semCom Γ Δ m n B
 
@@ -276,12 +287,12 @@ notation:40 Γ:41 "∣" Δ:41 "⊨" m:41 "~" n:41 "∶" B:41 => semCom Γ Δ m n
 
 theorem semVal.sym {Γ v w} {A : ValType} (h : Γ ⊨ v ~ w ∶ A) : Γ ⊨ w ~ v ∶ A :=
   λ hστ ↦ (h hστ.sym).sym
-theorem semCom.sym {Γ Δ m n} {B : ComType} (h : Γ ∣ Δ ⊨ m ~ n ∶ B) : Γ ∣ Δ ⊨ n ~ m ∶ B :=
+theorem semCom.sym {Γ δ Δ} {m n : Com δ} {B : ComType} (h : Γ ∣ Δ ⊨ m ~ n ∶ B) : Γ ∣ Δ ⊨ n ~ m ∶ B :=
   λ hστ _ _ hjs ↦ (h hστ.sym hjs.sym).sym
 
 theorem semVal.trans {Γ v₁ v₂ v₃} {A : ValType} (h₁₂ : Γ ⊨ v₁ ~ v₂ ∶ A) (h₂₃ : Γ ⊨ v₂ ~ v₃ ∶ A) : Γ ⊨ v₁ ~ v₃ ∶ A :=
   λ hστ ↦ by refine 𝒱.trans (h₁₂ hστ) (h₂₃ (semCtxt.trans hστ.sym hστ))
-theorem semCom.trans {Γ Δ m₁ m₂ m₃} {B : ComType} (h₁₂ : Γ ∣ Δ ⊨ m₁ ~ m₂ ∶ B) (h₂₃ : Γ ∣ Δ ⊨ m₂ ~ m₃ ∶ B) : Γ ∣ Δ ⊨ m₁ ~ m₃ ∶ B :=
+theorem semCom.trans {Γ δ Δ} {m₁ m₂ m₃ : Com δ} {B : ComType} (h₁₂ : Γ ∣ Δ ⊨ m₁ ~ m₂ ∶ B) (h₂₃ : Γ ∣ Δ ⊨ m₂ ~ m₃ ∶ B) : Γ ∣ Δ ⊨ m₁ ~ m₃ ∶ B :=
   λ hστ _ _ hjs ↦ by refine ℰ.trans (h₁₂ hστ hjs) (h₂₃ (semCtxt.trans hστ.sym hστ) (semDtxt.trans hjs.sym hjs))
 
 /-*---------------------------------------------
@@ -289,17 +300,17 @@ theorem semCom.trans {Γ Δ m₁ m₂ m₃} {B : ComType} (h₁₂ : Γ ∣ Δ �
   of syntactic typing wrt semantic equivalence
 ---------------------------------------------*-/
 
-theorem semCom.join {Γ Δ A B m₁ m₂ n₁ n₂} (hm : Γ ∷ A ∣ Δ ⊨ m₁ ~ m₂ ∶ B) (hn : Γ ∣ Δ ∷ A ↗ B ⊨ n₁ ~ n₂ ∶ B) :
+theorem semCom.join {Γ δ} {Δ : Dtxt δ} {A B m₁ m₂ n₁ n₂} (hm : Γ ∷ A ∣ Δ ⊨ m₁ ~ m₂ ∶ B) (hn : Γ ∣ Δ ∷ A ↗ B ⊨ n₁ ~ n₂ ∶ B) :
   Γ ∣ Δ ⊨ join m₁ n₁ ~ join m₂ n₂ ∶ B := by
-  intro σ τ hστ js₁ js₂ hjs
+  intro σ τ hστ js₁ js₂ hjs; simp; rw [← rejoin.eq_2, ← rejoin.eq_2]
   refine hn hστ (.cons hjs (λ {v w} hvw ↦ ?ihm))
   rw [substUnion, substUnion]
   exact hm (semCtxt.cons hvw hστ) hjs
 
-theorem semCom.jump {Γ : Ctxt} {Δ js₁ js₂ j A B} (mem : Δ ∋ j ∶ A ↗ B) (h : Δ ⊨ js₁ ~ js₂) :
+theorem semCom.jump {Γ : Ctxt} {δ} {Δ : Dtxt δ} {js₁ js₂ j A B} (mem : Δ ∋ j ∶ A ↗ B) (h : Δ ⊨ js₁ ~ js₂) :
   ∀ {σ τ v w}, Γ ⊨ σ ~ τ → (v, w) ∈ ⟦ A ⟧ᵛ →
   (rejoin (jump j v) js₁, rejoin (jump j w) js₂) ∈ ⟦ B ⟧ᵉ := by
-  induction h generalizing j A B
+  induction h generalizing A B
   case nil => cases mem
   case cons js₁ js₂ m n _ _ _ h _ =>
     cases mem
@@ -312,7 +323,7 @@ theorem semCom.jump {Γ : Ctxt} {Δ js₁ js₂ j A B} (mem : Δ ∋ j ∶ A ↗
 
 theorem soundness {Γ} :
   (∀ (v : Val) A, Γ ⊢ v ∶ A → Γ ⊨ v ~ v ∶ A) ∧
-  (∀ {Δ} (m : Com) B, Γ ∣ Δ ⊢ m ∶ B → Γ ∣ Δ ⊨ m ~ m ∶ B) := by
+  (∀ {δ Δ} (m : Com δ) B, Γ ∣ Δ ⊢ m ∶ B → Γ ∣ Δ ⊨ m ~ m ∶ B) := by
   refine ⟨λ v A h ↦ ?val, λ m B h ↦ ?com⟩
   mutual_induction h, h
   all_goals intro σ τ hστ
@@ -325,15 +336,15 @@ theorem soundness {Γ} :
   case force ih =>
     simp [𝒱] at ih
     let ⟨_, _, h, em, en⟩ := ih hστ
-    simp [em, en]; exact ℰ.bwdRejoin .π .π h
-  case lam ih =>
-    refine ℰ.bwdsRejoin .refl .refl (ℰ.lam (λ v w hA ↦ ?_))
+    simp [em, en]; exact ℰ.bwdRejoin0 .π .π h
+  case lam m _ _ _ ih =>
+    refine ℰ.bwdsRejoin0 (m' := (lam m)⦃σ⦄) (n' := (lam m)⦃τ⦄) .refl .refl (ℰ.lam (λ v w hA ↦ ?_))
     rw [substUnion, substUnion]
     exact ih (semCtxt.cons hA hστ) .nil
   case app ihm ihv =>
     let ⟨_ ,_, r₁, r₂, hAB⟩ := (ihm hστ .nil).lam_inv
     let hB := hAB _ _ (ihv hστ)
-    exact ℰ.bwdsRejoin (.trans' (Evals.app r₁) (.once .β)) (.trans' (Evals.app r₂) (.once .β)) hB
+    exact ℰ.bwdsRejoin0 (.trans' (Evals.app r₁) (.once .β)) (.trans' (Evals.app r₂) (.once .β)) hB
   case ret ih => exact ℰ.bwdsRejoin .refl .refl (ℰ.ret (ih hστ))
   case letin ihm ihn =>
     let ⟨v, w, r₁, r₂, hA⟩ := (ihm hστ .nil).ret_inv
@@ -356,12 +367,12 @@ theorem soundness {Γ} :
     exact ℰ.bwdsRejoin .refl .refl (ℰ.prod (ihm hστ .nil) (ihn hστ .nil))
   case fst ih =>
     let ⟨_, _, _, _, r₁, r₂, hB₁⟩ := (ih hστ .nil).fst
-    exact ℰ.bwdsRejoin (.trans' (Evals.fst r₁) (.once .π1)) (.trans' (Evals.fst r₂) (.once .π1)) hB₁
+    exact ℰ.bwdsRejoin0 (.trans' (Evals.fst r₁) (.once .π1)) (.trans' (Evals.fst r₂) (.once .π1)) hB₁
   case snd ih =>
     let ⟨_, _, _, _, r₁, r₂, hB₂⟩ := (ih hστ .nil).snd
-    exact ℰ.bwdsRejoin (.trans' (Evals.snd r₁) (.once .π2)) (.trans' (Evals.snd r₂) (.once .π2)) hB₂
+    exact ℰ.bwdsRejoin0 (.trans' (Evals.snd r₁) (.once .π2)) (.trans' (Evals.snd r₂) (.once .π2)) hB₂
   case join m n _ _ _ _ ihm ihn => exact semCom.join ihm ihn hστ hjs
   case jump mem _ ihv => exact semCom.jump mem hjs hστ (ihv hστ)
 
 def soundVal {Γ v} {A : ValType} : Γ ⊢ v ∶ A → Γ ⊨ v ~ v ∶ A := soundness.left v A
-def soundCom {Γ Δ m} {B : ComType} : Γ ∣ Δ ⊢ m ∶ B → Γ ∣ Δ ⊨ m ~ m ∶ B := soundness.right m B
+def soundCom {Γ δ} {Δ : Dtxt δ} {m} {B : ComType} : Γ ∣ Δ ⊢ m ∶ B → Γ ∣ Δ ⊨ m ~ m ∶ B := soundness.right m B
