CBPV/Evaluation.lean
@@ -10,21 +10,21 @@ open Nat Val Com
 section
 set_option hygiene false
 local infix:40 "⇒" => Eval
-inductive Eval : Com → Com → Prop where
+inductive Eval : ∀ {δ}, Com δ → Com δ → Prop where
   -- reduction steps
-  | π {m} : force (thunk m) ⇒ m
-  | β {m v} : app (lam m) v ⇒ m⦃v⦄
+  | π {δ m} : force (thunk m) ⇒ weakenJCom δ m
+  | β {δ m v} : app (lam m) v ⇒ weakenJCom δ (m⦃v⦄)
   | ζ {v m} : letin (ret v) m ⇒ m⦃v⦄
   | ιl {v m n} : case (inl v) m n ⇒ m⦃v⦄
   | ιr {v m n} : case (inr v) m n ⇒ n⦃v⦄
-  | π1 {m n} : fst (prod m n) ⇒ m
-  | π2 {m n} : snd (prod m n) ⇒ n
+  | π1 {δ m n} : fst (prod m n) ⇒ weakenJCom δ m
+  | π2 {δ m n} : snd (prod m n) ⇒ weakenJCom δ n
   | γ {m v} : join m (jump 0 v) ⇒ m⦃v⦄
   -- drop joins
   | ret {m v} : join m (ret v) ⇒ ret v
   | lam {m n} : join m (lam n) ⇒ lam n
   | prod {m n₁ n₂} : join m (prod n₁ n₂) ⇒ prod n₁ n₂
-  | join't {j m v} : join m (jump (j + 1) v) ⇒ jump j v
+  | join't {j m v} : join m (jump (j.succ) v) ⇒ (jump j v)
   -- congruence rules
   | app {m m' v} :
     m ⇒ m' →
@@ -49,76 +49,102 @@ inductive Eval : Com → Com → Prop where
 end
 infix:40 "⇒" => Eval
 
+namespace Eval
+
 -- Single-step evaluation is deterministic
-theorem Eval.det {m n₁ n₂} (r₁ : m ⇒ n₁) (r₂ : m ⇒ n₂) : n₁ = n₂ := by
-  induction r₁ generalizing n₂
+theorem det {δ} {m n₁ n₂ : Com δ} (r₁ : m ⇒ n₁) (r₂ : m ⇒ n₂) : n₁ = n₂ := by
+  induction r₁
+  case join't j _ _ =>
+    generalize e : Fin.succ j = j' at r₂
+    cases r₂
+    case γ => injection e; contradiction
+    case join v n r => cases r
+    case join't =>
+      injection e with e; injection e with e
+      cases j; subst e; rfl
   all_goals cases r₂; try rfl
   case fst.fst ih _ r | snd.snd ih _ r => rw [ih r]
   all_goals try apply_rules [appCong, letinCong, prodCong, joinCong]
   all_goals rename _ ⇒ _ => r; cases r
 
+-- Jump scope renaming preserves evaluation
+theorem renameJ {δ δ' m n} {ξ : Fin δ → Fin δ'} (r : m ⇒ n) : renameJCom ξ m ⇒ renameJCom ξ n := by
+  induction r generalizing δ' <;> simp
+  all_goals try rw [← renameJSubst]
+  all_goals try rw [renameWeakenJ]
+  all_goals constructor <;> apply_assumption
+
+theorem weakenJ {δ δ' m n} (r : m ⇒ n) : @weakenJCom δ δ' m ⇒ @weakenJCom δ δ' n := renameJ r
+
+end Eval
+
 /-*----------------------
   Multi-step evaluation
 ----------------------*-/
 
-@[reducible] def Evals := RTC Eval
+@[reducible] def Evals {δ} := RTC (@Eval δ)
 infix:40 "⇒⋆" => Evals
 
 namespace Evals
 
-theorem app {m n v} (r : m ⇒⋆ n) : app m v ⇒⋆ app n v := by
+theorem app {δ m n v} (r : m ⇒⋆ n) : @app δ m v ⇒⋆ @app δ n v := by
   induction r
   case refl => exact .refl
   case trans r _ ih => exact .trans (.app r) ih
 
-theorem letin {m m' n} (r : m ⇒⋆ m') : letin m n ⇒⋆ letin m' n := by
+theorem letin {δ m m' n} (r : m ⇒⋆ m') : @letin δ m n ⇒⋆ @letin δ m' n := by
   induction r
   case refl => exact .refl
   case trans r _ ih => exact .trans (.letin r) ih
 
-theorem fst {m m'} (r : m ⇒⋆ m') : fst m ⇒⋆ fst m' := by
+theorem fst {δ m m'} (r : m ⇒⋆ m') : @fst δ m ⇒⋆ @fst δ m' := by
   induction r
   case refl => exact .refl
   case trans r _ ih => exact .trans (.fst r) ih
 
-theorem snd {m m'} (r : m ⇒⋆ m') : snd m ⇒⋆ snd m' := by
+theorem snd {δ m m'} (r : m ⇒⋆ m') : @snd δ m ⇒⋆ @snd δ m' := by
   induction r
   case refl => exact .refl
   case trans r _ ih => exact .trans (.snd r) ih
 
-theorem join {m n n'} (r : n ⇒⋆ n') : join m n ⇒⋆ join m n' := by
+theorem join {δ m n n'} (r : n ⇒⋆ n') : @join δ m n ⇒⋆ @join δ m n' := by
   induction r
   case refl => exact .refl
   case trans r _ ih => exact .trans (.join r) ih
 
-theorem ret_inv {v m} (r : ret v ⇒⋆ m) : ret v = m := by
+theorem ret_inv {δ v m} (r : @ret δ v ⇒⋆ m) : ret v = m := by
   generalize e : ret v = n at r
   induction r generalizing v <;> subst e
   case refl => rfl
   case trans r => cases r
 
-theorem lam_inv {m n} (r : lam m ⇒⋆ n) : lam m = n := by
+theorem lam_inv {δ m n} (r : @lam δ m ⇒⋆ n) : lam m = n := by
   generalize e : lam m = m' at r
   induction r generalizing m <;> subst e
   case refl => rfl
   case trans r => cases r
 
-theorem prod_inv {m₁ m₂ n} (r : prod m₁ m₂ ⇒⋆ n) : prod m₁ m₂ = n := by
+theorem prod_inv {δ m₁ m₂ n} (r : @prod δ m₁ m₂ ⇒⋆ n) : prod m₁ m₂ = n := by
   generalize e : prod m₁ m₂ = m at r
   induction r generalizing m₁ m₂ <;> subst e
   case refl => rfl
   case trans r => cases r
 
-theorem jump_inv {j v n} (r : jump j v ⇒⋆ n) : jump j v = n := by
+theorem jump_inv {δ j v n} (r : @jump δ j v ⇒⋆ n) : jump j v = n := by
   generalize e : jump j v = m at r
   induction r generalizing j v <;> subst e
   case refl => rfl
   case trans r => cases r
 
+theorem weakenJ {δ δ' m n} (r : m ⇒⋆ n) : @weakenJCom δ δ' m ⇒⋆ @weakenJCom δ δ' n := by
+  induction r
+  case refl => rfl
+  case trans r _ ih => exact .trans (.weakenJ r) ih
+
 end Evals
 
 -- Multi-step reduction is confluent trivially by determinism
-theorem confluence {m n₁ n₂} (r₁ : m ⇒⋆ n₁) (r₂ : m ⇒⋆ n₂) : ∃ m', n₁ ⇒⋆ m' ∧ n₂ ⇒⋆ m' := by
+theorem confluence {δ} {m n₁ n₂ : Com δ} (r₁ : m ⇒⋆ n₁) (r₂ : m ⇒⋆ n₂) : ∃ m', n₁ ⇒⋆ m' ∧ n₂ ⇒⋆ m' := by
   induction r₁ generalizing n₂
   case refl => exact ⟨n₂, r₂, .refl⟩
   case trans r₁ rs₁ ih =>
@@ -131,82 +157,33 @@ theorem confluence {m n₁ n₂} (r₁ : m ⇒⋆ n₁) (r₂ : m ⇒⋆ n₂) :
 ----------------------------*-/
 
 @[simp]
-def nf : Com → Prop
+def nf {δ} : Com δ → Prop
   | lam _ | ret _ | prod _ _ => True
   | _ => False
 
-theorem nf.stepn't {m n} (nfm : nf m) : ¬ m ⇒ n := by
+theorem nf.stepn't {δ} {m n : Com δ} (nfm : nf m) : ¬ m ⇒ n := by
   cases m <;> simp at *
   all_goals intro r; cases r
 
-theorem nf.steps {m n} (nfm : nf m) (r : m ⇒⋆ n) : m = n := by
+theorem nf.steps {δ} {m n : Com δ} (nfm : nf m) (r : m ⇒⋆ n) : m = n := by
   cases r
   case refl => rfl
   case trans r _ => cases nfm.stepn't r
 
-def Norm (m n : Com) := m ⇒⋆ n ∧ nf n
+def Norm {δ} (m n : Com δ) := m ⇒⋆ n ∧ nf n
 infix:40 "⇓ₙ" => Norm
 
 namespace Norm
 
-@[refl] theorem refl {m} (nfm : nf m) : m ⇓ₙ m := by exists .refl
+@[refl] theorem refl {δ} {m : Com δ} (nfm : nf m) : m ⇓ₙ m := by exists .refl
 
-theorem bwds {m m' n} (r : m ⇒⋆ m') : m' ⇓ₙ n → m ⇓ₙ n
+theorem bwds {δ} {m m' n : Com δ} (r : m ⇒⋆ m') : m' ⇓ₙ n → m ⇓ₙ n
   | ⟨rn, nfn⟩ => ⟨.trans' r rn, nfn⟩
 
-theorem join {m n₁ n₂} : m ⇓ₙ n₁ → m ⇓ₙ n₂ → n₁ = n₂
+theorem join {δ} {m n₁ n₂ : Com δ} : m ⇓ₙ n₁ → m ⇓ₙ n₂ → n₁ = n₂
   | ⟨rn₁, nfn₁⟩, ⟨rn₂, nfn₂⟩ =>
     let ⟨n', rn₁', rn₂'⟩ := confluence rn₁ rn₂
     by rw [nfn₁.steps rn₁', nfn₂.steps rn₂']
-
-theorem dropJoin {n n'} : n ⇓ₙ n' → ∀ m, .join m n ⇓ₙ n'
-  | ⟨rn, nfn⟩, m => by
-    cases n' <;> simp at nfn
-    all_goals refine ⟨.trans' (Evals.join rn) (.once ?_), nfn⟩; constructor
-
-theorem join_inv' {m₁ m₂ n} (r : .join m₁ m₂ ⇓ₙ n) :
-  ∃ n', m₂ ⇒⋆ n' ∧ (nf n' ∨ ∃ j v, n' = jump j v) := by
-  let ⟨r, nfn⟩ := r
-  generalize e : Com.join m₁ m₂ = m₁' at r
-  induction r generalizing m₁ m₂ <;> subst e
-  case refl => cases nfn
-  case trans ih r =>
-    cases r
-    case ret | lam | prod => exact ⟨_, .refl, .inl ⟨⟩⟩
-    case γ | join't => exact ⟨_, .refl, .inr ⟨_, _, rfl⟩⟩
-    case join r rs =>
-      have ⟨_, rs, h⟩ := ih ⟨rs, nfn⟩ nfn rfl
-      exact ⟨_, .trans r rs, h⟩
-
-theorem join_inv {m₁ m₂ n} (r : .join m₁ m₂ ⇓ₙ n) :
-  m₂ ⇒⋆ n ∨ (∃ v, m₂ ⇒⋆ jump 0 v ∧ m₁⦃v⦄ ⇒⋆ n) ∨
-  (∃ j v, m₂ ⇒⋆ jump (j + 1) v ∧ renameJCom succ n = jump (j + 1) v) := by
-  let ⟨rn, nfn⟩ := r
-  match join_inv' r with
-  | ⟨n', rm₂, .inl nfn⟩ =>
-    have rm₂' := Evals.join (m := m₁) rm₂
-    cases n' <;> cases nfn
-    all_goals
-      have rn' := RTC.trans' rm₂' (.once (by constructor))
-      let ⟨_, r₁, r₂⟩ := confluence rn rn'
-      rw [← nfn.steps r₁] at r₂
-    case ret => rw [r₂.ret_inv] at rm₂; exact .inl rm₂
-    case lam => rw [r₂.lam_inv] at rm₂; exact .inl rm₂
-    case prod => rw [r₂.prod_inv] at rm₂; exact .inl rm₂
-  | ⟨_, rm₂, .inr ⟨_, _, e⟩⟩ =>
-    subst e
-    have rn' := Evals.join (m := m₁) rm₂
-    let ⟨_, r₁, r₂⟩ := confluence rn rn'
-    rw [← nfn.steps r₁] at r₂
-    cases r₂
-    case refl => cases nfn
-    case trans rj rn =>
-      cases rj
-      case join r => cases r
-      case γ => exact .inr (.inl ⟨_, rm₂, rn⟩)
-      case join't =>
-        rw [← Evals.jump_inv rn]
-        exact .inr (.inr ⟨_, _, rm₂, rfl⟩)
 
 end Norm
 
@@ -214,13 +191,13 @@ end Norm
   Strong normalization
 ---------------------*-/
 
-inductive SN : Com → Prop where
+inductive SN {δ} : Com δ → Prop where
   | sn : ∀ m, (∀ n, m ⇒ n → SN n) → SN m
 
-theorem SN.nf {m} (nfm : nf m) : SN m := by
+theorem SN.nf {δ m} (nfm : nf m) : @SN δ m := by
   constructor; intro n r; cases nfm.stepn't r
 
-theorem Evals.sn {m n} (r : m ⇒⋆ n) (nfn : nf n) : SN m := by
+theorem Evals.sn {δ m n} (r : m ⇒⋆ n) (nfn : nf n) : @SN δ m := by
   induction r
   case refl => exact .nf nfn
   case trans r _ ih => constructor; intro _ r'; rw [← Eval.det r r']; exact ih nfn
