CBPV/Syntax.lean
@@ -8,6 +8,12 @@ def cons {A : Type} (x : A) (ξ : Nat → A) : Nat → A
   | n + 1 => ξ n
 infixr:50 "+:" => cons
 
+@[simp]
+def consFin {A : Type} {δ : Nat} (x : A) (ξ : Fin δ → A) : Fin (δ + 1) → A
+  | ⟨0, _⟩ => x
+  | ⟨n + 1, lt⟩ => ξ ⟨n, lt_of_succ_lt_succ lt⟩
+infixr:50 "+::" => consFin
+
 /-*------
   Types
 ------*-/
@@ -35,33 +41,33 @@ inductive Val : Type where
   | unit : Val
   | inl : Val → Val
   | inr : Val → Val
-  | thunk : Com → Val
+  | thunk : Com 0 → Val
 
-inductive Com : Type where
-  | force : Val → Com
-  | lam : Com → Com
-  | app : Com → Val → Com
-  | ret : Val → Com
-  | letin : Com → Com → Com
-  | case : Val → Com → Com → Com
-  | prod : Com → Com → Com
-  | fst : Com → Com
-  | snd : Com → Com
-  | join : Com → Com → Com
-  | jump : Nat → Val → Com
+inductive Com : Nat → Type where
+  | force {δ} : Val → Com δ
+  | lam {δ} : Com 0 → Com δ
+  | app {δ} : Com 0 → Val → Com δ
+  | ret {δ} : Val → Com δ
+  | letin {δ} : Com 0 → Com δ → Com δ
+  | case {δ} : Val → Com δ → Com δ → Com δ
+  | prod {δ} : Com 0 → Com 0 → Com δ
+  | fst {δ} : Com 0 → Com δ
+  | snd {δ} : Com 0 → Com δ
+  | join {δ} : Com δ → Com (δ + 1) → Com δ
+  | jump {δ} : Fin δ → Val → Com δ
 end
 open Val Com
 
-theorem appCong {m m' v v'} : m = m' → v = v' → app m v = app m' v'
+theorem appCong {δ m m' v v'} : m = m' → v = v' → @app δ m v = @app δ m' v'
   | rfl, rfl => rfl
 
-theorem letinCong {m m' n n'} : m = m' → n = n' → letin m n = letin m' n'
+theorem letinCong {δ m m'} {n n' : Com δ} : m = m' → n = n' → letin m n = letin m' n'
   | rfl, rfl => rfl
 
-theorem prodCong {m m' n n'} : m = m' → n = n' → prod m n = prod m' n'
+theorem prodCong {δ m m' n n'} : m = m' → n = n' → @prod δ m n = @prod δ m' n'
   | rfl, rfl => rfl
 
-theorem joinCong {m m' n n'} : m = m' → n = n' → join m n = join m' n'
+theorem joinCong {δ} {m m' : Com δ} {n n'} : m = m' → n = n' → join m n = join m' n'
   | rfl, rfl => rfl
 
 /-*------------------
@@ -93,6 +99,28 @@ theorem liftSucc ξ : ∀ x, (lift ξ ∘ succ) x = (succ ∘ ξ) x := by
 theorem liftLiftSucc ξ : ∀ (x : Nat), (lift (lift ξ) ∘ lift succ) x = (lift succ ∘ (lift ξ)) x := by
   intro x; cases x <;> simp [lift]
 
+/-*-----------------------
+  Lifting jump renamings
+-----------------------*-/
+
+def liftJ {δ δ'} (ξ : Fin δ → Fin δ') : Fin (δ + 1) → Fin (δ' + 1) :=
+  0 +:: (Fin.succ ∘ ξ)
+
+-- Lifting respects jump renaming extensionality
+theorem liftJExt {δ₁ δ₂} (ξ ζ : Fin δ₁ → Fin δ₂) (h : ∀ j, ξ j = ζ j) : ∀ j, liftJ ξ j = liftJ ζ j
+  | .mk j lt => by cases j <;> simp [liftJ, h]
+
+-- Lifting identity jump renaming does nothing
+theorem liftJId {δ} (ξ : Fin δ → Fin δ) (h : ∀ j, ξ j = j) : ∀ j, liftJ ξ j = j
+  | ⟨j, _⟩ => by cases j <;> simp [liftJ, h]
+
+-- Lifting composes for jump renamings
+theorem liftJComp {δ₁ δ₂ δ₃} (ξ : Fin δ₂ → Fin δ₃) (ζ : Fin δ₁ → Fin δ₂) (ς : Fin δ₁ → Fin δ₃) (h : ∀ j, (ξ ∘ ζ) j = ς j) :
+  ∀ j, (liftJ ξ ∘ liftJ ζ) j = liftJ ς j
+  | .mk j lt => by
+    cases j <;> simp; rfl
+    case succ => simp [liftJ, Fin.succ, ← congrArg Fin.val (h _)]
+
 /-*-------------------
   Applying renamings
 -------------------*-/
@@ -107,7 +135,7 @@ def renameVal (ξ : Nat → Nat) : Val → Val
   | thunk m => thunk (renameCom ξ m)
 
 @[simp]
-def renameCom (ξ : Nat → Nat) : Com → Com
+def renameCom {δ} (ξ : Nat → Nat) : Com δ → Com δ
   | force v => force (renameVal ξ v)
   | lam m => lam (renameCom (lift ξ) m)
   | app m v => app (renameCom ξ m) (renameVal ξ v)
@@ -124,19 +152,19 @@ end
 -- Renaming extensionality
 theorem renameExt ξ ζ (h : ∀ x, ξ x = ζ x) :
   (∀ v, renameVal ξ v = renameVal ζ v) ∧
-  (∀ m, renameCom ξ m = renameCom ζ m) := by
+  (∀ {δ} (m : Com δ), renameCom ξ m = renameCom ζ m) := by
   refine ⟨λ v ↦ ?val, λ m ↦ ?com⟩
   mutual_induction v, m generalizing ξ ζ
   all_goals simp; try repeat' constructor
   all_goals apply_rules [liftExt]
 
-def renameValExt ξ ζ h := (renameExt ξ ζ h).left
-def renameComExt ξ ζ h := (renameExt ξ ζ h).right
+def renameValExt ξ ζ h := (@renameExt ξ ζ h).left
+def renameComExt {δ} ξ ζ h := @(renameExt ξ ζ h).right δ
 
 -- Applying identity renaming does nothing
 theorem renameId :
   (∀ v, renameVal id v = v) ∧
-  (∀ m, renameCom id m = m) := by
+  (∀ {δ} (m : Com δ), renameCom id m = m) := by
   refine ⟨λ v ↦ ?val, λ m ↦ ?com⟩
   mutual_induction v, m
   all_goals simp; try repeat' constructor
@@ -145,12 +173,12 @@ theorem renameId :
   all_goals apply_rules [liftId]
 
 def renameValId := renameId.left
-def renameComId := renameId.right
+def renameComId {δ} := @renameId.right δ
 
 -- Renamings compose
 theorem renameComp ξ ζ ς (h : ∀ x, (ξ ∘ ζ) x = ς x) :
   (∀ v, (renameVal ξ ∘ renameVal ζ) v = renameVal ς v) ∧
-  (∀ m, (renameCom ξ ∘ renameCom ζ) m = renameCom ς m) := by
+  (∀ {δ} (m : Com δ), (renameCom ξ ∘ renameCom ζ) m = renameCom ς m) := by
   refine ⟨λ v ↦ ?val, λ m ↦ ?comp⟩
   mutual_induction v, m generalizing ξ ζ ς
   all_goals simp; try repeat' constructor
@@ -159,17 +187,58 @@ theorem renameComp ξ ζ ς (h : ∀ x, (ξ ∘ ζ) x = ς x) :
 def renameValComp ξ ζ v : renameVal ξ (renameVal ζ v) = renameVal (ξ ∘ ζ) v :=
   (renameComp ξ ζ (ξ ∘ ζ) (λ _ ↦ rfl)).left v
 
-def renameComComp ξ ζ m : renameCom ξ (renameCom ζ m) = renameCom (ξ ∘ ζ) m :=
+def renameComComp {δ} ξ ζ (m : Com δ) : renameCom ξ (renameCom ζ m) = renameCom (ξ ∘ ζ) m :=
   (renameComp ξ ζ (ξ ∘ ζ) (λ _ ↦ rfl)).right m
 
--- Jump renamings
+/-*------------------------
+  Applying jump renamings
+------------------------*-/
+
 @[simp]
-def renameJCom (ξ : Nat → Nat) : Com → Com
+def renameJCom {δ δ'} (ξ : Fin δ → Fin δ') : Com δ → Com δ'
+  | force v => force v
+  | lam m => lam m
+  | app m v => app m v
+  | ret v => ret v
   | letin m n => letin m (renameJCom ξ n)
   | case v m n => case v (renameJCom ξ m) (renameJCom ξ n)
-  | join n m => join (renameJCom ξ n) (renameJCom (lift ξ) m)
+  | prod m n => prod m n
+  | fst m => fst m
+  | snd m => snd m
+  | join n m => join (renameJCom ξ n) (renameJCom (liftJ ξ) m)
   | jump j v => jump (ξ j) v
-  | m => m
+
+theorem renameJExt {δ₁ δ₂} (ξ ζ : Fin δ₁ → Fin δ₂) (h : ∀ x, ξ x = ζ x) m :
+  renameJCom ξ m = renameJCom ζ m := by
+  mutual_induction m generalizing δ₂ ξ ζ
+  all_goals simp; try constructor
+  all_goals apply_rules [liftJExt]
+
+theorem renameJId {δ} (m : Com δ) : renameJCom id m = m := by
+  mutual_induction m
+  all_goals simp; try repeat' constructor
+  all_goals try assumption
+  all_goals rw [renameJExt (liftJ id) id]
+  all_goals apply_rules [liftJId id (λ _ ↦ rfl)]
+
+theorem renameJComp {δ₁ δ₂ δ₃ m} (ξ : Fin δ₂ → Fin δ₃) (ζ : Fin δ₁ → Fin δ₂) :
+  renameJCom ξ (renameJCom ζ m) = renameJCom (ξ ∘ ζ) m := by
+  mutual_induction m generalizing δ₂ δ₃ ξ ζ <;> simp
+  all_goals try constructor
+  all_goals try apply_rules
+  case join ih =>
+    rw [renameJExt (liftJ (ξ ∘ ζ)) (liftJ ξ ∘ liftJ ζ) ?_]
+    . exact ih (liftJ ξ) (liftJ ζ)
+    . intro j; exact Eq.symm (liftJComp ξ ζ (ξ ∘ ζ) (λ _ ↦ rfl) j)
+
+@[reducible]
+def weakenJCom {δ} δ' : Com δ → Com (δ' + δ) := renameJCom (Fin.castLE (le_add_left δ δ'))
+
+theorem weakenJCom0 {m : Com 0} : weakenJCom 0 m = m :=
+  trans (renameJExt _ _ (λ _ ↦ rfl) m) (renameJId m)
+
+theorem renameWeakenJ {δ δ'} {ξ : Fin δ → Fin δ'} {m : Com 0} : renameJCom ξ (weakenJCom δ m) = weakenJCom δ' m := by
+  simp [weakenJCom]; rw [renameJComp, renameJExt _ _ (λ j ↦ by cases j.isLt)]
 
 /-*----------------------
   Lifting substitutions
@@ -238,7 +307,7 @@ def substVal (σ : Nat → Val) : Val → Val
   | thunk m => thunk (substCom σ m)
 
 @[simp]
-def substCom (σ : Nat → Val) : Com → Com
+def substCom {δ} (σ : Nat → Val) : Com δ → Com δ
   | force v => force (substVal σ v)
   | lam m => lam (substCom (⇑ σ) m)
   | app m v => app (substCom σ m) (substVal σ v)
@@ -258,50 +327,50 @@ notation:50 m "⦃" v "⦄" => substCom (v +: var) m
 -- Substitution extensionality
 theorem substExt σ τ (h : ∀ x, σ x = τ x) :
   (∀ v, substVal σ v = substVal τ v) ∧
-  (∀ m, substCom σ m = substCom τ m) := by
+  (∀ {δ} (m : Com δ), substCom σ m = substCom τ m) := by
   refine ⟨λ v ↦ ?val, λ m ↦ ?com⟩
   mutual_induction v, m generalizing σ τ
   all_goals simp; try repeat' constructor
   all_goals apply_rules [upExt]
 
 def substValExt σ τ h := (substExt σ τ h).left
-def substComExt σ τ h := (substExt σ τ h).right
+def substComExt {δ} σ τ h := @(substExt σ τ h).right δ
 
 -- Applying var "substitution" does nothing
 theorem substId σ (h : ∀ x, σ x = var x) :
   (∀ v, substVal σ v = v) ∧
-  (∀ m, substCom σ m = m) := by
+  (∀ {δ} (m : Com δ), substCom σ m = m) := by
   refine ⟨λ v ↦ ?val, λ m ↦ ?com⟩
   mutual_induction v, m generalizing σ
   all_goals simp; try repeat' constructor
   all_goals apply_rules [upId]
 
 def substValId := (substId var (λ _ ↦ rfl)).left
-def substComId := (substId var (λ _ ↦ rfl)).right
+def substComId {δ} := @(substId var (λ _ ↦ rfl)).right δ
 
 -- Substitution/renaming compositionality
 theorem substRename ξ σ τ (h : ∀ x, (σ ∘ ξ) x = τ x) :
   (∀ v, substVal σ (renameVal ξ v) = substVal τ v) ∧
-  (∀ m, substCom σ (renameCom ξ m) = substCom τ m) := by
+  (∀ {δ} (m : Com δ), substCom σ (renameCom ξ m) = substCom τ m) := by
   refine ⟨λ v ↦ ?val, λ m ↦ ?com⟩
   mutual_induction v, m generalizing ξ σ τ
   all_goals simp; try repeat' constructor
   all_goals apply_rules [upLift]
 
 def substRenameVal ξ σ := (substRename ξ σ (σ ∘ ξ) (λ _ ↦ rfl)).left
-def substRenameCom ξ σ := (substRename ξ σ (σ ∘ ξ) (λ _ ↦ rfl)).right
+def substRenameCom {δ} ξ σ := @(substRename ξ σ (σ ∘ ξ) (λ _ ↦ rfl)).right δ
 
 -- Renaming/substitution compositionality
 theorem renameSubst ξ σ τ (h : ∀ x, (renameVal ξ ∘ σ) x = τ x) :
   (∀ v, renameVal ξ (substVal σ v) = substVal τ v) ∧
-  (∀ m, renameCom ξ (substCom σ m) = substCom τ m) := by
+  (∀ {δ} (m : Com δ), renameCom ξ (substCom σ m) = substCom τ m) := by
   refine ⟨λ v ↦ ?val, λ m ↦ ?com⟩
   mutual_induction v, m generalizing ξ σ τ
   all_goals simp; try repeat' constructor
   all_goals apply_rules [upRename]
 
 def renameSubstVal ξ σ := (renameSubst ξ σ (renameVal ξ ∘ σ) (λ _ ↦ rfl)).left
-def renameSubstCom ξ σ := (renameSubst ξ σ (renameVal ξ ∘ σ) (λ _ ↦ rfl)).right
+def renameSubstCom {δ} ξ σ := @(renameSubst ξ σ (renameVal ξ ∘ σ) (λ _ ↦ rfl)).right δ
 
 -- Lifting commutes with substitution
 theorem upSubst ρ σ τ (h : ∀ x, (substVal ρ ∘ σ) x = τ x) :
@@ -318,19 +387,19 @@ theorem upSubst ρ σ τ (h : ∀ x, (substVal ρ ∘ σ) x = τ x) :
 -- Substitution compositionality
 theorem substComp ρ σ τ (h : ∀ x, (substVal ρ ∘ σ) x = τ x) :
   (∀ v, (substVal ρ ∘ substVal σ) v = substVal τ v) ∧
-  (∀ m, (substCom ρ ∘ substCom σ) m = substCom τ m) := by
+  (∀ {δ} (m : Com δ), (substCom ρ ∘ substCom σ) m = substCom τ m) := by
   refine ⟨λ v ↦ ?val, λ m ↦ ?com⟩
   mutual_induction v, m generalizing ρ σ τ
   all_goals simp; try repeat' constructor
   all_goals apply_rules [upSubst]
 
 def substValComp ρ σ := (substComp ρ σ (substVal ρ ∘ σ) (λ _ ↦ rfl)).left
-def substComComp ρ σ := (substComp ρ σ (substVal ρ ∘ σ) (λ _ ↦ rfl)).right
+def substComComp {δ} ρ σ := @(substComp ρ σ (substVal ρ ∘ σ) (λ _ ↦ rfl)).right δ
 
 -- Renamings are substitutions
 theorem renameToSubst ξ :
   (∀ v, renameVal ξ v = substVal (var ∘ ξ) v) ∧
-  (∀ m, renameCom ξ m = substCom (var ∘ ξ) m) := by
+  (∀ {δ} (m : Com δ), renameCom ξ m = substCom (var ∘ ξ) m) := by
   refine ⟨λ v ↦ ?val, λ m ↦ ?com⟩
   mutual_induction v, m generalizing ξ
   all_goals simp <;> try repeat' constructor
@@ -338,13 +407,18 @@ theorem renameToSubst ξ :
   all_goals apply_rules
 
 def renameToSubstVal ξ := (renameToSubst ξ).left
-def renameToSubstCom ξ := (renameToSubst ξ).right
+def renameToSubstCom {δ} ξ := @(renameToSubst ξ).right δ
 
 -- Join point renamings commute with substitution
-theorem renameJSubst ξ σ m : substCom σ (renameJCom ξ m) = renameJCom ξ (substCom σ m) := by
-  mutual_induction m generalizing ξ σ
+theorem renameJSubst {δ δ'} (ξ : Fin δ → Fin δ') σ (m : Com δ) :
+  substCom σ (renameJCom ξ m) = renameJCom ξ (substCom σ m) := by
+  mutual_induction m generalizing δ' ξ σ
   all_goals simp; try repeat' constructor
   all_goals apply_rules
+
+theorem weakenJSubst {δ δ'} σ (m : Com δ) :
+  substCom σ (weakenJCom δ' m) = weakenJCom δ' (substCom σ m) :=
+  renameJSubst _ σ m
 
 /-*-----------------------------------------------------
   Handy dandy derived renaming and substitution lemmas
@@ -357,17 +431,17 @@ theorem substDropVal v w : substVal (v +: var) (renameVal succ w) = w := by
     _ = substVal var w := by rw [substRenameVal]; rfl
     _ = w := by rw [substValId]
 
-theorem substDropCom v m : substCom (v +: var) (renameCom succ m) = m := by
+theorem substDropCom {δ} v (m : Com δ) : substCom (v +: var) (renameCom succ m) = m := by
   calc substCom (v +: var) (renameCom succ m)
     _ = substCom var m := by rw [substRenameCom]; rfl
     _ = m := by rw [substComId]
 
-theorem substDrop₂ σ v₁ v₂ m : substCom (v₁ +: v₂ +: σ) (renameCom (lift succ) m) = substCom (v₁ +: σ) m := by
+theorem substDrop₂ {δ} σ v₁ v₂ (m : Com δ) : substCom (v₁ +: v₂ +: σ) (renameCom (lift succ) m) = substCom (v₁ +: σ) m := by
   calc substCom (v₁ +: v₂ +: σ) (renameCom (lift succ) m)
     _ = substCom ((v₁ +: v₂ +: σ) ∘ lift succ) m   := by rw [substRenameCom]
     _ = substCom (v₁ +: σ) m                       := by rw [substComExt]; intro n; cases n <;> rfl
 
-theorem substUnion σ v m : substCom (v +: var) (substCom (⇑ σ) m) = substCom (v +: σ) m := by
+theorem substUnion {δ} σ v (m : Com δ) : substCom (v +: var) (substCom (⇑ σ) m) = substCom (v +: σ) m := by
   calc substCom (v +: var) (substCom (⇑ σ) m)
     _ = (substCom (v +: var) ∘ substCom (⇑ σ)) m := rfl
     _ = substCom (substVal (v +: var) ∘ (var 0 +: (renameVal succ ∘ σ))) m :=
@@ -376,7 +450,7 @@ theorem substUnion σ v m : substCom (v +: var) (substCom (⇑ σ) m) = substCom
       by apply substComExt; intro n; cases n <;> simp; rw [substDropVal]
 
 -- Helper for substUnion
-private theorem substUnion₂' σ v₁ v₂ m : substCom (substVal (v₁ +: v₂ +: var) ∘ (⇑ ⇑ σ)) m = substCom (v₁ +: v₂ +: σ) m := by
+private theorem substUnion₂' {δ} σ v₁ v₂ (m : Com δ) : substCom (substVal (v₁ +: v₂ +: var) ∘ (⇑ ⇑ σ)) m = substCom (v₁ +: v₂ +: σ) m := by
   apply substComExt
   intro n; cases n; simp [up]
   case succ n =>
@@ -386,7 +460,7 @@ private theorem substUnion₂' σ v₁ v₂ m : substCom (substVal (v₁ +: v₂
       have e x : (((v₁+:v₂+:var) ∘ succ) ∘ succ) x = var x := by rfl
       rw [substValExt _ _ e, substValId]
 
-theorem substUnion₂ σ v₁ v₂ m : substCom (v₁ +: v₂ +: var) (substCom (⇑ ⇑ σ) m) = substCom (v₁ +: v₂ +: σ) m := by
+theorem substUnion₂ {δ} σ v₁ v₂ (m : Com δ) : substCom (v₁ +: v₂ +: var) (substCom (⇑ ⇑ σ) m) = substCom (v₁ +: v₂ +: σ) m := by
   calc substCom (v₁ +: v₂ +: var) (substCom (⇑ ⇑ σ) m)
     _ = (substCom (v₁ +: v₂ +: var) ∘ substCom (⇑ ⇑ σ)) m := rfl
     _ = substCom (substVal (v₁ +: v₂ +: var) ∘ (⇑ ⇑ σ)) m := by rw [substComComp]
@@ -394,13 +468,13 @@ theorem substUnion₂ σ v₁ v₂ m : substCom (v₁ +: v₂ +: var) (substCom 
 
 /-* Pushing in lifts and ups through renamings *-/
 
-theorem renameLiftRename ξ m : renameCom (lift ξ) (renameCom succ m) = renameCom succ (renameCom ξ m) := by
+theorem renameLiftRename {δ} ξ (m : Com δ) : renameCom (lift ξ) (renameCom succ m) = renameCom succ (renameCom ξ m) := by
   calc renameCom (lift ξ) (renameCom succ m)
     _ = renameCom (lift ξ ∘ succ) m    := by rw [renameComComp]
     _ = renameCom (succ ∘ ξ) m         := by rw [renameComExt]; exact liftSucc ξ
     _ = renameCom succ (renameCom ξ m) := by rw [renameComComp]
 
-theorem renameLiftLiftRename ξ m : renameCom (lift (lift ξ)) (renameCom (lift succ) m) = renameCom (lift succ) (renameCom (lift ξ) m) := by
+theorem renameLiftLiftRename {δ} ξ (m : Com δ) : renameCom (lift (lift ξ)) (renameCom (lift succ) m) = renameCom (lift succ) (renameCom (lift ξ) m) := by
   calc renameCom (lift (lift ξ)) (renameCom (lift succ) m)
     _ = renameCom (lift (lift ξ) ∘ lift succ) m      := by rw [renameComComp]
     _ = renameCom (lift succ ∘ lift ξ) m             := by rw [renameComExt]; exact liftLiftSucc ξ
@@ -412,26 +486,26 @@ theorem renameUpSubstVal σ v : substVal (⇑ σ) (renameVal succ v) = renameVal
   _ = substVal (renameVal succ ∘ σ) v := by rw [substValExt _ _ (upSucc σ)]
   _ = renameVal succ (substVal σ v)   := by rw [renameSubstVal]
 
-theorem renameUpSubstCom σ m : substCom (⇑ σ) (renameCom succ m) = renameCom succ (substCom σ m) := by
+theorem renameUpSubstCom {δ} σ (m : Com δ) : substCom (⇑ σ) (renameCom succ m) = renameCom succ (substCom σ m) := by
   calc substCom (⇑ σ) (renameCom succ m)
   _ = substCom (⇑ σ ∘ succ) m         := by rw [substRenameCom]
   _ = substCom (renameVal succ ∘ σ) m := by rw [substComExt _ _ (upSucc σ)]
   _ = renameCom succ (substCom σ m)   := by rw [renameSubstCom]
 
-theorem renameUpUpSubst σ m : substCom (⇑ ⇑ σ) (renameCom (lift succ) m) = renameCom (lift succ) (substCom (⇑ σ) m) := by
+theorem renameUpUpSubst {δ} σ (m : Com δ) : substCom (⇑ ⇑ σ) (renameCom (lift succ) m) = renameCom (lift succ) (substCom (⇑ σ) m) := by
   calc substCom (⇑ ⇑ σ) (renameCom (lift succ) m)
     _ = substCom (⇑ ⇑ σ ∘ lift succ) m             := by rw [substRenameCom]
     _ = substCom (renameVal (lift succ) ∘ (⇑ σ)) m := by rw [substComExt _ _ (upUpSucc σ)]
     _ = renameCom (lift succ) (substCom (⇑ σ) m)   := by rw [renameSubstCom]
 
-theorem renameUpSubstCons σ v m : substCom (⇑ (v +: σ)) (renameCom (lift succ) m) = substCom (⇑ σ) m := by
+theorem renameUpSubstCons {δ} σ v (m : Com δ) : substCom (⇑ (v +: σ)) (renameCom (lift succ) m) = substCom (⇑ σ) m := by
   calc substCom (⇑ (v +: σ)) (renameCom (lift succ) m)
     _ = substCom (⇑ (v +: σ) ∘ lift succ) m := by rw [substRenameCom]
     _ = substCom (⇑ σ) m                    := by rw [substComExt]; intro n; cases n <;> rfl
 
 /-* Terrible name but extremely specific lemma for Equivalence.letLet/.letCase I will never use again *-/
 
-theorem renameDropSubst σ m v : ((renameCom (lift succ) m)⦃⇑⇑ σ⦄⦃⇑ (v +: var)⦄) = (m⦃⇑ σ⦄) := by
+theorem renameDropSubst {δ} σ (m : Com δ) v : ((renameCom (lift succ) m)⦃⇑⇑ σ⦄⦃⇑ (v +: var)⦄) = (m⦃⇑ σ⦄) := by
   calc (renameCom (lift succ) m)⦃⇑⇑ σ⦄⦃⇑ (v +: var)⦄
     _ = (renameCom (lift succ) (m ⦃⇑ σ⦄)⦃⇑ (v +: var)⦄) := by rw [renameUpUpSubst]
     _ = (renameCom (lift succ) (m ⦃⇑ σ⦄)⦃var 0 +: renameVal succ v +: var ∘ succ⦄)
@@ -457,38 +531,18 @@ inductive Ctxt.In : Nat → ValType → Ctxt → Prop where
   | there {Γ x A B} : In x A Γ → In (succ x) A (Γ ∷ B)
 notation:40 Γ:41 "∋" x:41 "∶" A:41 => Ctxt.In x A Γ
 
-@[simp]
-def Ctxt.length : Ctxt → Nat
-  | .nil => 0
-  | .cons Γ _ => Γ.length + 1
-
-theorem Ctxt.inLength {Γ x A} (h : Γ ∋ x ∶ A) : x < Γ.length := by
-  induction h
-  case here => simp
-  case there ih => simp [ih]
-
 /-* Jump contexts *-/
 
-inductive Dtxt : Type where
-  | nil : Dtxt
-  | cons : Dtxt → ValType → ComType → Dtxt
+inductive Dtxt : Nat → Type where
+  | nil : Dtxt 0
+  | cons {δ} : Dtxt δ → ValType → ComType → Dtxt (δ + 1)
 notation:50 "⬝" => Dtxt.nil
 notation:50 Δ:51 "∷" A:51 "↗" B:51 => Dtxt.cons Δ A B
 
-inductive Dtxt.In : Nat → ValType → ComType → Dtxt → Prop where
+inductive Dtxt.In : ∀ {δ}, Fin δ → ValType → ComType → Dtxt δ → Prop where
   | here {Δ A B} : In 0 A B (Δ ∷ A ↗ B)
-  | there {Δ j A A' B B'} : In j A B Δ → In (succ j) A B (Δ ∷ A' ↗ B')
+  | there {Δ j A A' B B'} : In j A B Δ → In j.succ A B (Δ ∷ A' ↗ B')
 notation:40 Δ:41 "∋" j:41 "∶" A:41 "↗" B:41 => Dtxt.In j A B Δ
-
-@[simp]
-def Dtxt.length : Dtxt → Nat
-  | .nil => 0
-  | .cons Δ _ _ => Δ.length + 1
-
-theorem Dtxt.inLength {Δ j A B} (h : Δ ∋ j ∶ A ↗ B) : j < Δ.length := by
-  induction h
-  case here => simp
-  case there ih => simp [ih]
 
 /-*----------------------
   Well-scoped renamings
@@ -512,15 +566,15 @@ theorem wRenameLift {ξ : Nat → Nat} {Γ Δ A}
 
 /-* Jump renamings *-/
 
-def wRenameJ (ξ : Nat → Nat) (Δ Φ : Dtxt) := ∀ j A B, Δ ∋ j ∶ A ↗ B → Φ ∋ ξ j ∶ A ↗ B
+def wRenameJ {δ δ'} (ξ : Fin δ → Fin δ') (Δ : Dtxt δ) (Φ : Dtxt δ') := ∀ j A B, Δ ∋ j ∶ A ↗ B → Φ ∋ ξ j ∶ A ↗ B
 notation:40 Φ "⊢" ξ:41 "∶" Δ:41 => wRenameJ ξ Δ Φ
 
-theorem wRenameJSucc {Δ A B} : Δ ∷ A ↗ B ⊢ succ ∶ Δ := by
+theorem wRenameJSucc {δ} {Δ : Dtxt δ} {A B} : Δ ∷ A ↗ B ⊢ Fin.succ ∶ Δ := by
   intro j A' B' mem; constructor; assumption
 
-theorem wRenameJLift {ξ : Nat → Nat} {Δ Φ : Dtxt} {A B}
+theorem wRenameJLift {δ δ'} {ξ : Fin δ → Fin δ'} {Δ : Dtxt δ} {Φ : Dtxt δ'} {A B}
   (h : Φ ⊢ ξ ∶ Δ) :
-  Φ ∷ A ↗ B ⊢ lift ξ ∶ Δ ∷ A ↗ B := by
+  Φ ∷ A ↗ B ⊢ liftJ ξ ∶ Δ ∷ A ↗ B := by
   intro x A' B' mem
   cases mem with
   | here => exact Dtxt.In.here
