CBPV/Antirenaming.lean
@@ -4,370 +4,103 @@ import CBPV.Typing
 
 open Nat Val Com
 
-/-*------------------------------------------------
-  Well-scopedness with respect to jump variables:
-  * ScopeComJ δ m says that the jump variables
-    in m are bounded by δ (jump context length)
-  * ScopeValJ v helps assert that any thunks in v
-    are closed wrt jump variables
-------------------------------------------------*-/
-
-mutual
-inductive ScopeValJ : Val → Prop where
-  | var {x} : ScopeValJ (var x)
-  | unit : ScopeValJ unit
-  | inl {v} : ScopeValJ v → ScopeValJ (inl v)
-  | inr {v} : ScopeValJ v → ScopeValJ (inr v)
-  | thunk {m} : ScopeComJ 0 m → ScopeValJ (thunk m)
-
-inductive ScopeComJ : Nat → Com → Prop where
-  | force {δ v} : ScopeValJ v → ScopeComJ δ (force v)
-  | lam {δ m} : ScopeComJ 0 m → ScopeComJ δ (lam m)
-  | app {δ m v} : ScopeComJ 0 m → ScopeValJ v → ScopeComJ δ (app m v)
-  | ret {δ v} : ScopeValJ v → ScopeComJ δ (ret v)
-  | letin {δ m n} : ScopeComJ 0 m → ScopeComJ δ n → ScopeComJ δ (letin m n)
-  | case {δ v m n} : ScopeValJ v → ScopeComJ δ m → ScopeComJ δ n → ScopeComJ δ (case v m n)
-  | prod {δ m n} : ScopeComJ 0 m → ScopeComJ 0 n → ScopeComJ δ (prod m n)
-  | fst {δ m} : ScopeComJ 0 m → ScopeComJ δ (fst m)
-  | snd {δ m} : ScopeComJ 0 m → ScopeComJ δ (snd m)
-  | join {δ m n} : ScopeComJ δ m → ScopeComJ (δ + 1) n → ScopeComJ δ (join m n)
-  | jump {δ j v} : j < δ → ScopeValJ v → ScopeComJ δ (jump j v)
-end
-
-@[simp, reducible]
-def ScopeSubstJ (σ : Nat → Val) := ∀ x, ScopeValJ (σ x)
-
-/-* Well-typedness implies jump well-scopedness *-/
-
-theorem wtScopeJ {Γ} :
-  (∀ {v} {A : ValType}, Γ ⊢ v ∶ A → ScopeValJ v) ∧
-  (∀ {Δ m} {B : ComType}, Γ ∣ Δ ⊢ m ∶ B → ScopeComJ (Δ.length) m) := by
-  refine ⟨λ hv ↦ ?val, λ hm ↦ ?com⟩
-  mutual_induction hv, hm
-  all_goals constructor <;> try assumption
-  case com.jump mem _ ih => exact Dtxt.inLength mem
-
-theorem ValWt.scopeJ {Γ v} {A : ValType} : Γ ⊢ v ∶ A → ScopeValJ v := wtScopeJ.left
-theorem ComWt.scopeJ {Γ Δ m B} : Γ ∣ Δ ⊢ m ∶ B → ScopeComJ (Δ.length) m := wtScopeJ.right
-
-/-* Jump scopes can be weakened *-/
-
-theorem ScopeComJ.weaken {δ δ' m} (h : ScopeComJ δ m) : ScopeComJ (δ + δ') m := by
-  mutual_induction h <;> constructor <;> try assumption
-  case join ih => rw [Nat.add_right_comm]; exact ih
-  case jump ltδ _ => exact Nat.lt_add_right δ' ltδ
-theorem ScopeComJ.weaken0 {δ m} (h : ScopeComJ 0 m) : ScopeComJ δ m :=
-  by rw [← Nat.zero_add δ]; exact h.weaken
-
-/-* Jump-renaming a computation in an empty jump scope does nothing *-/
-
-@[simp]
-def lifts (ξ : Nat → Nat) : Nat → (Nat → Nat)
-  | 0 => ξ
-  | n + 1 => lift (lifts ξ n)
-
-theorem liftsId {ξ δ j} (ltδ : j < δ) : lifts ξ δ j = j := by
-  induction δ generalizing j; contradiction
-  case succ ih =>
-    cases j <;> simp [lift]
-    exact ih (Nat.lt_of_add_lt_add_right ltδ)
-
-theorem ScopeComJ.renameScopeJ {ξ δ m} (h : ScopeComJ δ m) : renameJCom (lifts ξ δ) m = m := by
-  mutual_induction h generalizing ξ <;> simp
-  case letin ih => exact ih
-  case case ih₁ ih₂ => exact ⟨ih₁, ih₂⟩
-  case jump ltδ _ => exact liftsId ltδ
-  case join ih₁ ih₂ => exact ⟨ih₁, ih₂⟩
-theorem ScopeComJ.renameScopeJ0 {ξ m} : ScopeComJ 0 m → renameJCom ξ m = m := renameScopeJ
-
-/-* Renaming and substitution preserve jump scoping *-/
-
-theorem renameScope {ξ} :
-  (∀ {v}, ScopeValJ v → ScopeValJ (renameVal ξ v)) ∧
-  (∀ {δ m}, ScopeComJ δ m → ScopeComJ δ (renameCom ξ m)) := by
-  refine ⟨λ hv ↦ ?val, λ hm ↦ ?com⟩
-  mutual_induction hv, hm generalizing ξ
-  all_goals constructor <;> apply_assumption
-
-theorem ScopeSubstJ.lift {σ} (hσ : ScopeSubstJ σ) : ScopeSubstJ (⇑ σ) := by
-  intro n; cases n <;> simp [up]; constructor
-  case succ n => exact renameScope.left (hσ n)
-
-theorem substScope {σ} (hσ : ScopeSubstJ σ) :
-  (∀ {v}, ScopeValJ v → ScopeValJ (v⦃σ⦄)) ∧
-  (∀ {δ m}, ScopeComJ δ m → ScopeComJ δ (m⦃σ⦄)) := by
-  refine ⟨λ hv ↦ ?val, λ hm ↦ ?com⟩
-  mutual_induction hv, hm generalizing σ
-  case var x => exact hσ x
-  all_goals constructor <;> try apply_rules [ScopeSubstJ.lift]
-
-theorem ScopeComJ.subst {δ σ m} (hσ : ScopeSubstJ σ) : ScopeComJ δ m → ScopeComJ δ (m⦃σ⦄) :=
-  (substScope hσ).right
-
-theorem ScopeComJ.subst1 {δ m v} (hv : ScopeValJ v) (hm : ScopeComJ δ m) : ScopeComJ δ (m⦃v⦄) := by
-  refine (substScope ?_).right hm
-  intro n; cases n; exact hv; constructor
-
-theorem Eval.scopeJ {δ m n} (r : m ⇒ n) (h : ScopeComJ δ m) : ScopeComJ δ n := by
-  induction r generalizing δ
-  case π =>
-    cases h with | force h =>
-    cases h with | thunk h =>
-    exact h.weaken0
-  case β =>
-    cases h with | app hlam hv =>
-    cases hlam with | lam h =>
-    exact h.weaken0.subst1 hv
-  case ζ =>
-    cases h with | letin hret h =>
-    cases hret with | ret hv =>
-    exact h.subst1 hv
-  case ιl =>
-    cases h with | case hinl hl hr =>
-    cases hinl with | inl hv =>
-    exact hl.subst1 hv
-  case ιr =>
-    cases h with | case hinr hl hr =>
-    cases hinr with | inr hv =>
-    exact hr.subst1 hv
-  case π1 =>
-    cases h with | fst h =>
-    cases h with | prod h₁ h₂ =>
-    exact h₁.weaken0
-  case π2 =>
-    cases h with | snd h =>
-    cases h with | prod h₁ h₂ =>
-    exact h₂.weaken0
-  case γ =>
-    cases h with | join h hjump =>
-    cases hjump with | jump _ hv =>
-    exact h.subst1 hv
-  case ret =>
-    cases h with | join _ hret =>
-    cases hret with | ret hv =>
-    exact .ret hv
-  case lam =>
-    cases h with | join h₁ h₂ =>
-    cases h₂ with | lam h₂ =>
-    exact .lam h₂
-  case prod =>
-    cases h with | join h₁ h₂ =>
-    cases h₂ with | prod h₂ h₃ =>
-    exact .prod h₂ h₃
-  case join't =>
-    cases h with | join h₁ h₂ =>
-    cases h₂ with | jump ltδ hv =>
-    exact .jump (lt_of_succ_lt_succ ltδ) hv
-  case app ih =>
-    cases h with | app hm hv =>
-    exact .app (ih hm) hv
-  case letin ih =>
-    cases h with | letin h₁ h₂ =>
-    exact .letin (ih h₁) h₂
-  case fst ih =>
-    cases h with | fst h =>
-    exact .fst (ih h)
-  case snd ih =>
-    cases h with | snd h =>
-    exact .snd (ih h)
-  case join ih =>
-    cases h with | join h₁ h₂ =>
-    refine .join h₁ (ih h₂)
-
-/-* Evaluation respects jump renaming *-/
-
-theorem Eval.renameJ {ξ δ m n} (h : ScopeComJ δ m) (r : m ⇒ n) : renameJCom ξ m ⇒ renameJCom ξ n := by
-  induction r generalizing ξ δ
-  all_goals simp; try rw [← renameJSubst]
-  case π =>
-    cases h with | force h =>
-    cases h with | thunk h =>
-    rw [h.renameScopeJ0]; constructor
-  case β =>
-    cases h with | app hlam hv =>
-    cases hlam with | lam h =>
-    rw [h.renameScopeJ0]; constructor
-  case π1 =>
-    cases h with | fst h =>
-    cases h with | prod h₁ h₂ =>
-    rw [h₁.renameScopeJ0]; constructor
-  case π2 =>
-    cases h with | snd h =>
-    cases h with | prod h₁ h₂ =>
-    rw [h₂.renameScopeJ0]; constructor
-  case join ih =>
-    cases h with | join _ h =>
-    exact .join (ih h)
-  all_goals constructor <;> assumption
-
 /-*-----------------------------------------------------------
   Antirenaming: If a jump-renamed m reduces to n,
   then n must be some renamed computation that m reduces to;
   we require that m be well-scoped wrt jump variables.
 -----------------------------------------------------------*-/
 
-theorem antirenameJ {ξ δ m n'} (h : ScopeComJ δ m) (r : renameJCom ξ m ⇒ n') :
+theorem antirenameJ {δ δ' m n'} {ξ : Fin δ → Fin δ'} (r : renameJCom ξ m ⇒ n') :
   ∃ n, n' = renameJCom ξ n ∧ m ⇒ n := by
   generalize e : renameJCom ξ m = m' at r
-  induction r generalizing ξ δ m
+  induction r generalizing δ m
   case π =>
     cases m <;> injection e
-    cases h with | force h =>
-    case force m e =>
-      cases m <;> injection e
-      cases h with | thunk h =>
-      case thunk e =>
-        subst e; exact ⟨_, h.renameScopeJ0.symm, .π⟩
+    case force v _ e =>
+      cases v <;> injection e; subst_vars
+      exact ⟨_, renameWeakenJ.symm, .π⟩
   case β =>
     cases m <;> injection e
-    cases h with | app h =>
-    case app m v em ev _ =>
-      cases m <;> injection em
-      cases h with | lam h =>
-      case lam em =>
-        subst em ev; refine ⟨_, ?_, .β⟩
-        rw [← renameJSubst, h.renameScopeJ0]
+    case app m _ _ em _ =>
+      cases m <;> injection em; subst_vars
+      exact ⟨_, renameWeakenJ.symm, .β⟩
   case ζ =>
     cases m <;> injection e
-    case letin m₁ m₂ em₁ em₂ =>
-      cases m₁ <;> injection em₁
-      case ret v ev =>
-        subst ev em₂
-        exact ⟨_, renameJSubst ξ (v +: var) m₂, .ζ⟩
-  case ιl =>
+    case letin m₁ m₂ _ em₁ _ =>
+      cases m₁ <;> injection em₁; subst_vars
+      exact ⟨_, renameJSubst ξ (_ +: var) m₂, .ζ⟩
+  case ιl | ιr =>
     cases m <;> injection e
-    case case v m₁ m₂ ev em₁ em₂ =>
-      cases v <;> injection ev
-      case inl v ev =>
-        subst ev em₁ em₂
-        exact ⟨_, renameJSubst ξ (v +: var) m₁, .ιl⟩
-  case ιr =>
+    case case v _ _ _ ev _ _ =>
+      cases v <;> injection ev; subst_vars
+      exact ⟨_, renameJSubst ξ (_ +: var) _, by constructor⟩
+  case π1 | π2 =>
     cases m <;> injection e
-    case case v m₁ m₂ ev em₁ em₂ =>
-      cases v <;> injection ev
-      case inr v ev =>
-        subst ev em₁ em₂
-        exact ⟨_, renameJSubst ξ (v +: var) m₂, .ιr⟩
-  case π1 =>
+    case _ m _ e =>
+      cases m <;> injection e; subst_vars
+      exact ⟨_, renameWeakenJ.symm, by constructor⟩
+  case ret | lam | prod =>
     cases m <;> injection e
-    cases h with | fst h =>
-    case fst m e =>
-      cases m <;> injection e
-      cases h with | prod h₁ h₂ =>
-      case prod em₁ em₂ =>
-        subst em₁ em₂; exact ⟨_, h₁.renameScopeJ0.symm, .π1⟩
-  case π2 =>
-    cases m <;> injection e
-    cases h with | snd h =>
-    case snd m e =>
-      cases m <;> injection e
-      cases h with | prod h₁ h₂ =>
-      case prod em₁ em₂ =>
-        subst em₁ em₂; exact ⟨_, h₂.renameScopeJ0.symm, .π2⟩
+    case join m₁ m₂ _ em₁ em₂ =>
+      cases m₂ <;> injection em₂; subst_vars
+      exact ⟨_, rfl, by constructor⟩
+  case app r _ | letin r _ | fst r _ | snd r _ =>
+    cases m <;> injection e; subst_vars
+    exact ⟨_, rfl, by constructor; exact r⟩
   case γ =>
     cases m <;> injection e
-    case join m₁ m₂ em₁ em₂ =>
+    case join m₁ m₂ _ em₁ em₂ =>
       cases m₂ <;> injection em₂
-      case jump j v ej ev =>
-        cases j <;> injection ej
+      case jump v j _ ej ev =>
         subst ev em₁
-        exact ⟨_, renameJSubst ξ (v +: var) m₁, .γ⟩
-  case ret =>
-    cases m <;> injection e
-    case join m₁ m₂ em₁ em₂ =>
-      cases m₂ <;> injection em₂
-      case ret v ev =>
-        subst ev em₁; exact ⟨_, rfl, .ret⟩
-  case lam =>
-    cases m <;> injection e
-    case join m₁ m₂ em₁ em₂ =>
-      cases m₂ <;> injection em₂
-      case lam m₂ em₂ =>
-        subst em₁ em₂; exact ⟨_, rfl, .lam⟩
+        match j with
+        | ⟨0, _⟩ => exact ⟨_, renameJSubst ξ (v +: var) m₁, .γ⟩
+        | ⟨j + 1, _⟩ => cases ej
   case join't =>
     cases m <;> injection e
-    case join m₁ m₂ em₁ em₂ =>
+    case join m₁ m₂ _ em₁ em₂ =>
       cases m₂ <;> injection em₂
-      case jump j v ej ev =>
-      cases j <;> injection ej
-      case succ j ej =>
-        subst ev ej; exact ⟨_, rfl, .join't⟩
-  case prod =>
-    cases m <;> injection e
-    case join m₁ m₂ em₁ em₂ =>
-      cases m₂ <;> injection em₂
-      case prod n₁ n₂ en₁ en₂ =>
-        subst en₁ en₂; exact ⟨_, rfl, .prod⟩
-  case app =>
-    cases m <;> injection e
-    cases h with | app h =>
-    case app ih m v em ev _ =>
-      subst em ev
-      have e : renameJCom ξ m = m := h.renameScopeJ0
-      let ⟨n, en, r⟩ := ih h e; subst en
-      refine ⟨_, ?_, .app r⟩; simp
-      exact (r.scopeJ h).renameScopeJ0
-  case letin =>
-    cases m <;> injection e
-    cases h with | letin h₁ h₂ =>
-    case letin ih m₁ m₂ em₁ em₂ =>
-      subst em₁ em₂
-      have e : renameJCom ξ m₁ = m₁ := h₁.renameScopeJ0
-      let ⟨n, en, r⟩ := ih h₁ e; subst en
-      refine ⟨_, ?_, .letin r⟩; simp
-      exact (r.scopeJ h₁).renameScopeJ0
-  case fst =>
-    cases m <;> injection e
-    case fst ih m e =>
-      subst e
-      cases h with | fst h =>
-      have e : renameJCom ξ m = m := h.renameScopeJ0
-      let ⟨n, en, r⟩ := ih h e; subst en
-      refine ⟨_, ?_, .fst r⟩; simp
-      exact (r.scopeJ h).renameScopeJ0
-  case snd =>
-    cases m <;> injection e
-    case snd ih m e =>
-      subst e
-      cases h with | snd h =>
-      have e : renameJCom ξ m = m := h.renameScopeJ0
-      let ⟨n, en, r⟩ := ih h e; subst en
-      refine ⟨_, ?_, .snd r⟩; simp
-      exact (r.scopeJ h).renameScopeJ0
+      case jump v j _ ej ev =>
+      subst ev
+      match j with
+      | ⟨0, _⟩ => cases ej
+      | ⟨j + 1, lt⟩ =>
+        rw [← Fin.succ_mk _ _ (lt_of_succ_lt_succ lt)]
+        simp [liftJ] at ej; subst ej
+        exact ⟨_, rfl, .join't⟩
   case join =>
     cases m <;> injection e
-    case join ih m₁ m₂ em₁ em₂ =>
+    case join ih m₁ m₂ _ em₁ em₂ =>
+      let ⟨m₂', em₂, r⟩ := ih em₂
       subst em₁ em₂
-      cases h with | join _ h =>
-      let ⟨m₂', em₂, r⟩ := ih h rfl; subst em₂
       exact ⟨_, rfl, .join r⟩
 
 /-* Corollary: A jump-weakened join body can drop the join point *-/
 
-theorem Eval.wkJoin {δ js m₁ m₂ m} (h : ScopeComJ δ m₂) (r : .rejoin (.join m₁ (renameJCom succ m₂)) js ⇒ m) :
-  (m = .rejoin m₂ js) ∨ (∃ m₂', m₂ ⇒ m₂' ∧ m = .rejoin (.join m₁ (renameJCom succ m₂')) js) := by
+theorem Eval.wkJoin {δ} {js : J δ} {m₁ m₂ m} (r : .rejoin (.join m₁ (renameJCom Fin.succ m₂)) js ⇒ m) :
+  (m = .rejoin m₂ js) ∨ (∃ m₂', m₂ ⇒ m₂' ∧ m = .rejoin (.join m₁ (renameJCom Fin.succ m₂')) js) := by
   let ⟨_, r, e⟩ := r.rejoin_inv
-  generalize erename : renameJCom succ m₂ = m₂' at r
+  generalize erename : renameJCom Fin.succ m₂ = m₂' at r
   cases r
   case join r =>
     subst erename
-    let ⟨n, en, rn⟩ := antirenameJ h r
+    let ⟨n, en, rn⟩ := antirenameJ r
     subst en; exact .inr ⟨_, rn, e⟩
   all_goals cases m₂ <;> injection erename
   case γ ej _ => cases ej
   case ret e' | lam e' => subst e'; exact .inl e
   case prod e₁ e₂ => subst e₁ e₂; exact .inl e
-  case join't ej ev => injection ej with ej; subst ej ev; exact .inl e
+  case join't ej ev => rw [Fin.succ_inj.mp ej]; subst ev; exact .inl e
 
-theorem Norm.wkJoin {δ js m₁ m₂ n} (h : ScopeComJ δ m₂) (r : rejoin (.join m₁ (renameJCom succ m₂)) js ⇓ₙ n) :
-  ∃ m₂', m₂ ⇒⋆ m₂' ∧ rejoin (.join m₁ (renameJCom succ m₂)) js ⇒⋆ rejoin m₂' js ∧ rejoin m₂' js ⇒⋆ n := by
+theorem Norm.wkJoin {δ} {js : J δ} {m₁ m₂ n} (r : rejoin (.join m₁ (renameJCom Fin.succ m₂)) js ⇓ₙ n) :
+  ∃ m₂', m₂ ⇒⋆ m₂' ∧ rejoin (.join m₁ (renameJCom Fin.succ m₂)) js ⇒⋆ rejoin m₂' js ∧ rejoin m₂' js ⇒⋆ n := by
   cases r with | _ rn nfn =>
-  generalize e : rejoin (.join m₁ (renameJCom succ m₂)) js = m at rn
+  generalize e : rejoin (.join m₁ (renameJCom Fin.succ m₂)) js = m at rn
   induction rn generalizing m₂
   case refl => subst e; cases nfn.rejoin't (by simp)
   case trans r rs ih =>
     subst e
-    match r.wkJoin h with
+    match r.wkJoin with
     | .inl e =>
       subst e
       let ⟨_, r, e⟩ := r.rejoin_inv
@@ -375,5 +108,5 @@ theorem Norm.wkJoin {δ js m₁ m₂ n} (h : ScopeComJ δ m₂) (r : rejoin (.jo
       exact .rejoin (.once r)
     | .inr ⟨n, rn, en⟩ =>
       subst en
-      have ⟨_, rn', rjoin, rs⟩ := ih (rn.scopeJ h) nfn rfl
-      refine ⟨_, .trans rn rn', .trans (.rejoin (.join (rn.renameJ h))) rjoin, rs⟩
+      have ⟨_, rn', rjoin, rs⟩ := ih nfn rfl
+      refine ⟨_, .trans rn rn', .trans (.rejoin (.join rn.renameJ)) rjoin, rs⟩
