CBPV/CBN.lean
@@ -183,7 +183,7 @@ section
 set_option hygiene false
 local notation:40 "⟦" t:41 "⟧ᵗ" => transTerm t
 @[simp]
-def transTerm : CBN.Term → Com
+def transTerm : CBN.Term → Com 0
   | .var s => .force (.var s)
   | .unit => .ret .unit
   | .lam t => .lam (⟦ t ⟧ᵗ)
@@ -206,14 +206,14 @@ section
 set_option hygiene false
 local notation:40 "⟦" k:41 "⟧ᴷ" => transK k
 @[simp]
-def transK : CBN.K → K
-  | [] => []
-  | .app u :: k   => .app (.thunk (⟦ u ⟧ᵗ)) :: (⟦ k ⟧ᴷ)
+def transK : CBN.K → K 0
+  | [] => .nil
+  | .app u :: k   => .app (.thunk (⟦ u ⟧ᵗ)) (⟦ k ⟧ᴷ)
   | .case t u :: k => .letin (.case (.var 0)
                         (renameCom (lift succ) (⟦ t ⟧ᵗ))
-                        (renameCom (lift succ) (⟦ u ⟧ᵗ))) :: (⟦ k ⟧ᴷ)
-  | .fst :: k => .fst :: (⟦ k ⟧ᴷ)
-  | .snd :: k => .snd :: (⟦ k ⟧ᴷ)
+                        (renameCom (lift succ) (⟦ u ⟧ᵗ))) (⟦ k ⟧ᴷ)
+  | .fst :: k => .fst (⟦ k ⟧ᴷ)
+  | .snd :: k => .snd (⟦ k ⟧ᴷ)
 end
 notation:40 "⟦" k:41 "⟧ᴷ" => transK k
 
@@ -221,7 +221,7 @@ notation:40 "⟦" k:41 "⟧ᴷ" => transK k
 section
 set_option hygiene false
 local infix:40 "↦ₙ" => transTerm'
-inductive transTerm' : CBN.Term → Com → Prop where
+inductive transTerm' : CBN.Term → Com 0 → Prop where
   | var {s} : .var s ↦ₙ .force (.var s)
   | unit : .unit ↦ₙ .ret .unit
   | lam {t m} : t ↦ₙ m → .lam t ↦ₙ .lam m
@@ -278,7 +278,7 @@ theorem transRename {ξ t m} (h : t ↦ₙ m) : CBN.rename ξ t ↦ₙ renameCom
 
 theorem transUp {σ : Nat → CBN.Term} {σ' : Nat → Val}
   (h : ∀ x, σ x ↦ₙ .force (σ' x)) : ∀ x, (⇑ σ) x ↦ₙ .force ((⇑ σ') x) := by
-  have e {ξ v} : .force (renameVal ξ v) = renameCom ξ (.force v) := rfl
+  have e {ξ v} : .force (renameVal ξ v) = renameCom ξ (@Com.force 0 v) := rfl
   intro n; cases n
   case zero => exact .var
   case succ n => simp [up]; rw [e]; exact transRename (h n)
@@ -297,13 +297,16 @@ theorem transSubstSingle {t u} : CBN.subst (u +: .var) t ↦ₙ (⟦t⟧ᵗ) ⦃
 
 /-* Translation preserves machine semantics *-/
 
-theorem simulation {t u k k'} (r : ⟨t, k⟩ ⤳ₙ ⟨u, k'⟩) : ∃ m, ⟨⟦ t ⟧ᵗ, ⟦ k ⟧ᴷ⟩ ⤳⋆ ⟨m, ⟦ k' ⟧ᴷ⟩ ∧ u ↦ₙ m := by
+theorem simulation {t u k k'} (r : ⟨t, k⟩ ⤳ₙ ⟨u, k'⟩) : ∃ m, ⟨0, ⟦ t ⟧ᵗ, ⟦ k ⟧ᴷ⟩ ⤳⋆ ⟨0, m, ⟦ k' ⟧ᴷ⟩ ∧ u ↦ₙ m := by
   generalize et : (t, k)  = ck  at r
   generalize eu : (u, k') = ck' at r
   induction r
   all_goals injection et with et ek; subst et ek
   all_goals injection eu with eu ek; subst eu ek
-  case β t u => exact ⟨⟦ t ⟧ᵗ ⦃ .thunk (⟦ u ⟧ᵗ) ⦄, .once .β, transSubstSingle⟩
+  case β t u =>
+    have r := @Step.β 0 (⟦ t ⟧ᵗ) (.thunk (⟦ u ⟧ᵗ)) (⟦ k' ⟧ᴷ)
+    rw [weakenJCom0] at r
+    exact ⟨⟦ t ⟧ᵗ ⦃ .thunk (⟦ u ⟧ᵗ) ⦄, .once r, transSubstSingle⟩
   case ιl s t _ =>
     refine ⟨⟦ t ⟧ᵗ ⦃ .thunk (⟦ s ⟧ᵗ)⦄, ?_, transSubstSingle⟩
     calc
@@ -316,8 +319,8 @@ theorem simulation {t u k k'} (r : ⟨t, k⟩ ⤳ₙ ⟨u, k'⟩) : ∃ m, ⟨�
       _ ⤳ _ := .ζ
       _ ⤳ _ := by exact .ιr
       _ = _ := by rw [substUnion, substDrop₂]
-  case π1 => exact ⟨_, .once .π1, transTransTerm⟩
-  case π2 => exact ⟨_, .once .π2, transTransTerm⟩
+  case π1 => refine ⟨_, .once .π1, ?_⟩; rw [weakenJCom0]; exact transTransTerm
+  case π2 => refine ⟨_, .once .π2, ?_⟩; rw [weakenJCom0]; exact transTransTerm
   case app => exact ⟨_, .once .app, transTransTerm⟩
   case case => exact ⟨_, .once .letin, transTransTerm⟩
   case fst => exact ⟨_, .once .fst, transTransTerm⟩
