CBPV/Commutation.lean
@@ -3,7 +3,7 @@ import CBPV.Antirenaming
 
 open Nat ValType ComType Val Com
 
-theorem letLet {Γ Δ n m m' A} {B : ComType}
+theorem letLet {Γ δ} {Δ : Dtxt δ} {A n m m'} {B : ComType}
   (hlet : Γ ∣ ⬝ ⊢ letin n m ∶ F A)
   (hm' : Γ ∷ A ∣ Δ ⊢ m' ∶ B) :
   Γ ∣ Δ ⊨ letin (letin n m) m' ~ letin n (letin m (renameCom (lift succ) m')) ∶ B := by
@@ -29,13 +29,14 @@ theorem letLet {Γ Δ n m m' A} {B : ComType}
   have goal := soundCom hm' (semCtxt.cons hA hστ) hjs
   refine ℰ.bwds (.rejoin r₁') (.rejoin r₂') goal
 
-theorem appLet {Γ Δ n m v A B}
+theorem appLet {Γ δ} {Δ : Dtxt δ} {n m v A B}
   (hlet : Γ ∣ ⬝ ⊢ letin n m ∶ Arr A B)
   (hv : Γ ⊢ v ∶ A) :
   Γ ∣ Δ ⊨ app (letin n m) v ~ letin n (app m (renameVal succ v)) ∶ B := by
   intro σ τ hστ js₁ js₂ hjs
   let ⟨n₁, n₂, r₁, r₂, hB⟩ := (soundCom hlet hστ .nil).lam_inv
-  have r₁' : app ((letin n m)⦃σ⦄) (v⦃σ⦄) ⇒⋆ n₁⦃v⦃σ⦄⦄ := .trans' r₁.app (.once .β)
+  have r₁' : app ((letin n m)⦃σ⦄) (v⦃σ⦄) ⇒⋆ n₁⦃v⦃σ⦄⦄ := by
+    rw [← @weakenJCom0 (n₁⦃v⦃σ⦄⦄)]; exact .trans' r₁.app (.once .β)
   simp only [substCom] at *
   cases hlet with | letin hn hm =>
   let ⟨w₁, w₂, _, rw₂, hA'⟩ := (soundCom hn hστ .nil).ret_inv
@@ -45,7 +46,7 @@ theorem appLet {Γ Δ n m v A B}
     _ ⇒  m⦃w₂ +: τ⦄ := by rw [← substUnion]; exact .ζ
     _ ⇒⋆ lam m₂ := rm₂
   let ⟨_, rlam₁, rlam₂⟩ := confluence r₂ rlet
-  rw [← rlam₂.lam_inv] at rlam₁; injection rlam₁.lam_inv with e; subst e
+  rw [← rlam₂.lam_inv] at rlam₁; injection rlam₁.lam_inv with _ e; subst e
   clear rlet rlam₁ rlam₂
   have r₂' : letin (n⦃τ⦄) (app (m⦃⇑ τ⦄) (renameVal succ v⦃⇑ τ⦄))
       ⇒⋆ n₂⦃v⦃τ⦄⦄ := calc
@@ -54,15 +55,17 @@ theorem appLet {Γ Δ n m v A B}
     _ = app (m⦃w₂ +: τ⦄) (v⦃τ⦄)
       := by simp only [substCom]; rw [substUnion, renameUpSubstVal, substDropVal]
     _ ⇒⋆ app (lam n₂) (v⦃τ⦄) := rm₂.app
-    _ ⇒  n₂⦃v⦃τ⦄⦄ := .β
+    _ ⇒  weakenJCom 0 (n₂⦃v⦃τ⦄⦄) := .β
+    _ ⇒⋆ n₂⦃v⦃τ⦄⦄ := by rw [weakenJCom0]
   exact ℰ.bwdsRejoin r₁' r₂' (hB _ _ (soundVal hv hστ))
 
-theorem fstLet {Γ Δ n m B₁ B₂}
+theorem fstLet {Γ δ} {Δ : Dtxt δ} {n m B₁ B₂}
   (hlet : Γ ∣ ⬝ ⊢ letin n m ∶ Prod B₁ B₂) :
   Γ ∣ Δ ⊨ fst (letin n m) ~ letin n (fst m) ∶ B₁ := by
   intro σ τ hστ js₁ js₂ hjs
   let ⟨n₁, _, n₂, _, r₁, r₂, hB₁⟩ := (soundCom hlet hστ .nil).fst
-  have r₁' : fst ((letin n m)⦃σ⦄) ⇒⋆ n₁ := .trans' r₁.fst (.once .π1)
+  have r₁' : fst ((letin n m)⦃σ⦄) ⇒⋆ n₁ := by
+    rw [← @weakenJCom0 n₁]; exact .trans' r₁.fst (.once .π1)
   simp only [substCom] at *
   cases hlet with | letin hn hm =>
   let ⟨w₁, w₂, _, rw₂, hA'⟩ := (soundCom hn hστ .nil).ret_inv
@@ -72,22 +75,24 @@ theorem fstLet {Γ Δ n m B₁ B₂}
     _ ⇒  m⦃w₂ +: τ⦄              := by rw [← substUnion]; exact .ζ
     _ ⇒⋆ prod m₂ _               := r₂'
   let ⟨_, rprod₁, rprod₂⟩ := confluence r₂ rlet
-  rw [← rprod₂.prod_inv] at rprod₁; injection rprod₁.prod_inv with e₁ e₂; subst e₁ e₂
+  rw [← rprod₂.prod_inv] at rprod₁; injection rprod₁.prod_inv with _ e₁ e₂; subst e₁ e₂
   clear rlet rprod₁ rprod₂
   have r₂' : letin (n⦃τ⦄) (fst (m⦃⇑ τ⦄)) ⇒⋆ n₂ := calc
     _ ⇒⋆ letin (ret w₂) (fst (m⦃⇑ τ⦄)) := rw₂.letin
     _ ⇒  fst (m⦃⇑ τ⦄⦃w₂⦄)              := .ζ
     _ =  fst (m⦃w₂ +: τ⦄)              := by rw [substUnion]
     _ ⇒⋆ fst (prod n₂ _)               := r₂'.fst
-    _ ⇒  n₂                            := .π1
+    _ ⇒  weakenJCom 0 n₂               := .π1
+    _ ⇒⋆ n₂                            := by rw [weakenJCom0]
   exact ℰ.bwdsRejoin r₁' r₂' hB₁
 
-theorem sndLet {Γ Δ n m B₁ B₂}
+theorem sndLet {Γ δ} {Δ : Dtxt δ} {n m B₁ B₂}
   (hlet : Γ ∣ ⬝ ⊢ letin n m ∶ Prod B₁ B₂) :
   Γ ∣ Δ ⊨ snd (letin n m) ~ letin n (snd m) ∶ B₂ := by
   intro σ τ hστ js₁ js₂ hjs
   let ⟨_, n₁, _, n₂, r₁, r₂, hB₂⟩ := (soundCom hlet hστ .nil).snd
-  have r₁' : snd ((letin n m)⦃σ⦄) ⇒⋆ n₁ := .trans' r₁.snd (.once .π2)
+  have r₁' : snd ((letin n m)⦃σ⦄) ⇒⋆ n₁ := by
+    rw [← @weakenJCom0 n₁]; exact .trans' r₁.snd (.once .π2)
   simp only [substCom] at *
   cases hlet with | letin hn hm =>
   let ⟨w₁, w₂, _, rw₂, hA'⟩ := (soundCom hn hστ .nil).ret_inv
@@ -97,17 +102,18 @@ theorem sndLet {Γ Δ n m B₁ B₂}
     _ ⇒  m⦃w₂ +: τ⦄              := by rw [← substUnion]; exact .ζ
     _ ⇒⋆ prod m₂ _               := r₂'
   let ⟨_, rprod₁, rprod₂⟩ := confluence r₂ rlet
-  rw [← rprod₂.prod_inv] at rprod₁; injection rprod₁.prod_inv with e₁ e₂; subst e₁ e₂
+  rw [← rprod₂.prod_inv] at rprod₁; injection rprod₁.prod_inv with _ e₁ e₂; subst e₁ e₂
   clear rlet rprod₁ rprod₂
   have r₂' : letin (n⦃τ⦄) (snd (m⦃⇑ τ⦄)) ⇒⋆ n₂ := calc
     _ ⇒⋆ letin (ret w₂) (snd (m⦃⇑ τ⦄)) := rw₂.letin
     _ ⇒  snd (m⦃⇑ τ⦄⦃w₂⦄)              := .ζ
     _ =  snd (m⦃w₂ +: τ⦄)              := by rw [substUnion]
     _ ⇒⋆ snd (prod _ n₂)               := r₂'.snd
-    _ ⇒  n₂                            := .π2
+    _ ⇒  weakenJCom 0 n₂               := .π2
+    _ ⇒⋆ n₂                            := by rw [weakenJCom0]
   exact ℰ.bwdsRejoin r₁' r₂' hB₂
 
-theorem letCase {Γ Δ v m₁ m₂ n A} {B : ComType}
+theorem letCase {Γ δ} {Δ : Dtxt δ} {v m₁ m₂ n A} {B : ComType}
   (hcase : Γ ∣ ⬝ ⊢ case v m₁ m₂ ∶ F A)
   (hn : Γ ∷ A ∣ Δ ⊢ n ∶ B) :
   Γ ∣ Δ ⊨ letin (case v m₁ m₂) n
@@ -127,7 +133,7 @@ theorem letCase {Γ Δ v m₁ m₂ n A} {B : ComType}
       _ ⇒ m₁⦃w₂ +: τ⦄ := by rw [← substUnion]; exact .ιl
       _ ⇒⋆ ret n₂     := rn₂
     let ⟨_, rret₁, rret₂⟩ := confluence rv₂ rcase
-    rw [← rret₂.ret_inv] at rret₁; injection rret₁.ret_inv with e; subst e
+    rw [← rret₂.ret_inv] at rret₁; injection rret₁.ret_inv with _ e; subst e
     clear rcase rret₁ rret₂
     have r₂' : case (inl w₂)
                     (letin (m₁⦃⇑τ⦄) (renameCom (lift succ) n⦃⇑⇑τ⦄))
@@ -147,7 +153,7 @@ theorem letCase {Γ Δ v m₁ m₂ n A} {B : ComType}
       _ ⇒ m₂⦃w₂ +: τ⦄ := by rw [← substUnion]; exact .ιr
       _ ⇒⋆ ret n₂     := rn₂
     let ⟨_, rret₁, rret₂⟩ := confluence rv₂ rcase
-    rw [← rret₂.ret_inv] at rret₁; injection rret₁.ret_inv with e; subst e
+    rw [← rret₂.ret_inv] at rret₁; injection rret₁.ret_inv with _ e; subst e
     clear rcase rret₁ rret₂
     have r₂' : case (inr w₂)
                     (letin (m₁⦃⇑τ⦄) (renameCom (lift succ) n⦃⇑⇑τ⦄))
@@ -161,13 +167,14 @@ theorem letCase {Γ Δ v m₁ m₂ n A} {B : ComType}
     have goal := soundCom hn (semCtxt.cons hA hστ) hjs
     exact ℰ.bwds (.rejoin r₁') (.rejoin r₂') goal
 
-theorem appCase {Γ Δ v w m₁ m₂ A B}
+theorem appCase {Γ δ} {Δ : Dtxt δ} {v w m₁ m₂ A B}
   (hcase : Γ ∣ ⬝ ⊢ case v m₁ m₂ ∶ Arr A B)
   (hw : Γ ⊢ w ∶ A) :
   Γ ∣ Δ ⊨ app (case v m₁ m₂) w ~ case v (app m₁ (renameVal succ w)) (app m₂ (renameVal succ w)) ∶ B := by
   intro σ τ hστ js₁ js₂ hjs
   let ⟨n₁, n₂, r₁, r₂, hB₁⟩ := (soundCom hcase hστ .nil).lam_inv
-  have r₁' : app ((case v m₁ m₂)⦃σ⦄) (w⦃σ⦄) ⇒⋆ n₁⦃w⦃σ⦄⦄ := .trans' r₁.app (.once .β)
+  have r₁' : app ((case v m₁ m₂)⦃σ⦄) (w⦃σ⦄) ⇒⋆ n₁⦃w⦃σ⦄⦄ := by
+    rw [← @weakenJCom0 (n₁⦃w⦃σ⦄⦄)]; exact .trans' r₁.app (.once .β)
   simp only [substCom] at *
   cases hcase with | case hv hm₁ hm₂ =>
   let hv := soundVal hv hστ; unfold 𝒱 at hv
@@ -177,7 +184,7 @@ theorem appCase {Γ Δ v w m₁ m₂ A B}
     let ⟨_, _, _, r₂', _⟩ := (soundCom hm₁ (semCtxt.cons hA₁ hστ) .nil).lam_inv
     let ⟨_, rlam₁, r'⟩ := confluence r₂ (.once .ιl); rw [substUnion] at r'
     let ⟨_, rlam₂, r'⟩ := confluence r₂' r'; rw [← rlam₂.lam_inv] at r'
-    injection Evals.lam_inv (.trans' rlam₁ r') with en₂; subst en₂
+    injection Evals.lam_inv (.trans' rlam₁ r') with _ en₂; subst en₂
     clear rlam₁ rlam₂ r' r₁; clear r'
     have r₂' :
       case (.inl v₂) (app (m₁⦃⇑ τ⦄) (renameVal succ w⦃⇑ τ⦄)) (app (m₂⦃⇑ τ⦄) (renameVal succ w⦃⇑ τ⦄))
@@ -185,15 +192,16 @@ theorem appCase {Γ Δ v w m₁ m₂ A B}
       _ ⇒  app (m₁⦃⇑ τ⦄) (renameVal succ w⦃⇑ τ⦄) ⦃v₂⦄ := .ιl
       _ =  app (m₁⦃v₂ +: τ⦄) (w⦃τ⦄)
         := by simp only [substCom]; rw [substUnion, renameUpSubstVal, substDropVal]
-      _ ⇒⋆ app (lam n₂) (w⦃τ⦄) := r₂'.app
-      _ ⇒  n₂⦃w⦃τ⦄⦄ := .β
+      _ ⇒⋆ app (lam n₂) (w⦃τ⦄)     := r₂'.app
+      _ ⇒  weakenJCom 0 (n₂⦃w⦃τ⦄⦄) := .β
+      _ ⇒⋆ n₂⦃w⦃τ⦄⦄                := by rw [weakenJCom0]
     exact ℰ.bwdsRejoin r₁' r₂' (hB₁ _ _ (soundVal hw hστ))
   | .inr ⟨v₁, v₂, hA₂, e₁, e₂⟩ =>
     rw [e₂]; rw [e₂] at r₂
     let ⟨_, _, _, r₂', _⟩ := (soundCom hm₂ (semCtxt.cons hA₂ hστ) .nil).lam_inv
     let ⟨_, rlam₁, r'⟩ := confluence r₂ (.once .ιr); rw [substUnion] at r'
     let ⟨_, rlam₂, r'⟩ := confluence r₂' r'; rw [← rlam₂.lam_inv] at r'
-    injection Evals.lam_inv (.trans' rlam₁ r') with en₂; subst en₂
+    injection Evals.lam_inv (.trans' rlam₁ r') with _ en₂; subst en₂
     clear rlam₁ rlam₂ r' r₁; clear r'
     have r₂' :
       case (.inr v₂) (app (m₁⦃⇑ τ⦄) (renameVal succ w⦃⇑ τ⦄)) (app (m₂⦃⇑ τ⦄) (renameVal succ w⦃⇑ τ⦄))
@@ -201,16 +209,18 @@ theorem appCase {Γ Δ v w m₁ m₂ A B}
       _ ⇒  app (m₂⦃⇑ τ⦄) (renameVal succ w⦃⇑ τ⦄) ⦃v₂⦄ := .ιr
       _ =  app (m₂⦃v₂ +: τ⦄) (w⦃τ⦄)
         := by simp only [substCom]; rw [substUnion, renameUpSubstVal, substDropVal]
-      _ ⇒⋆ app (lam n₂) (w⦃τ⦄) := r₂'.app
-      _ ⇒  n₂⦃w⦃τ⦄⦄ := .β
+      _ ⇒⋆ app (lam n₂) (w⦃τ⦄)     := r₂'.app
+      _ ⇒  weakenJCom 0 (n₂⦃w⦃τ⦄⦄) := .β
+      _ ⇒⋆ n₂⦃w⦃τ⦄⦄                := by rw [weakenJCom0]
     exact ℰ.bwdsRejoin r₁' r₂' (hB₁ _ _ (soundVal hw hστ))
 
-theorem fstCase {Γ Δ v m₁ m₂ B₁ B₂}
+theorem fstCase {Γ δ} {Δ : Dtxt δ} {v m₁ m₂ B₁ B₂}
   (hcase : Γ ∣ ⬝ ⊢ case v m₁ m₂ ∶ Prod B₁ B₂) :
   Γ ∣ Δ ⊨ fst (case v m₁ m₂) ~ case v (fst m₁) (fst m₂) ∶ B₁ := by
   intro σ τ hστ js₁ js₂ hjs
   let ⟨n₁, _, n₂, _, r₁, r₂, hB₁⟩ := (soundCom hcase hστ .nil).fst
-  have r₁' : fst ((case v m₁ m₂)⦃σ⦄) ⇒⋆ n₁ := .trans' r₁.fst (.once .π1)
+  have r₁' : fst ((case v m₁ m₂)⦃σ⦄) ⇒⋆ n₁ := by
+    rw [← @weakenJCom0 n₁]; exact .trans' r₁.fst (.once .π1)
   simp only [substCom] at *
   cases hcase with | case hv hm₁ hm₂ =>
   let hv := soundVal hv hστ; unfold 𝒱 at hv
@@ -220,36 +230,39 @@ theorem fstCase {Γ Δ v m₁ m₂ B₁ B₂}
     let ⟨_, _, _, _, _, r₂', _⟩ := (soundCom hm₁ (semCtxt.cons hA₁ hστ) .nil).fst
     let ⟨_, rprod₁, r'⟩ := confluence r₂ (.once .ιl); rw [substUnion] at r'
     let ⟨_, rprod₂, r'⟩ := confluence r₂' r'; rw [← rprod₂.prod_inv] at r'
-    injection Evals.prod_inv (.trans' rprod₁ r') with en₁ en₂; subst en₁ en₂
+    injection Evals.prod_inv (.trans' rprod₁ r') with _ en₁ en₂; subst en₁ en₂
     clear rprod₁ rprod₂ r' r₁; clear r'
     have r₂' :
       case (inl v₂) (fst (m₁⦃⇑ τ⦄)) (fst (m₂⦃⇑ τ⦄)) ⇒⋆ n₂ := calc
       _ ⇒  fst (m₁⦃⇑ τ⦄)⦃v₂⦄ := .ιl
       _ =  fst (m₁⦃v₂ +: τ⦄) := by simp only [substCom]; rw [substUnion]
       _ ⇒⋆ fst (prod n₂ _)   := r₂'.fst
-      _ ⇒ n₂                 := .π1
+      _ ⇒  weakenJCom 0 n₂   := .π1
+      _ ⇒⋆ n₂                := by rw [weakenJCom0]
     exact ℰ.bwdsRejoin r₁' r₂' hB₁
   | .inr ⟨v₁, v₂, hA₂, e₁, e₂⟩ =>
     rw [e₂]; rw [e₂] at r₂
     let ⟨_, _, _, _, _, r₂', _⟩ := (soundCom hm₂ (semCtxt.cons hA₂ hστ) .nil).fst
     let ⟨_, rprod₁, r'⟩ := confluence r₂ (.once .ιr); rw [substUnion] at r'
     let ⟨_, rprod₂, r'⟩ := confluence r₂' r'; rw [← rprod₂.prod_inv] at r'
-    injection Evals.prod_inv (.trans' rprod₁ r') with en₁ en₂; subst en₁ en₂
+    injection Evals.prod_inv (.trans' rprod₁ r') with _ en₁ en₂; subst en₁ en₂
     clear rprod₁ rprod₂ r' r₁; clear r'
     have r₂' :
       case (inr v₂) (fst (m₁⦃⇑ τ⦄)) (fst (m₂⦃⇑ τ⦄)) ⇒⋆ n₂ := calc
       _ ⇒  fst (m₂⦃⇑ τ⦄)⦃v₂⦄ := .ιr
       _ =  fst (m₂⦃v₂ +: τ⦄) := by simp only [substCom]; rw [substUnion]
       _ ⇒⋆ fst (prod n₂ _)   := r₂'.fst
-      _ ⇒ n₂                 := .π1
+      _ ⇒  weakenJCom 0 n₂   := .π1
+      _ ⇒⋆ n₂                := by rw [weakenJCom0]
     exact ℰ.bwdsRejoin r₁' r₂' hB₁
 
-theorem sndCase {Γ Δ v m₁ m₂ B₁ B₂}
+theorem sndCase {Γ δ} {Δ : Dtxt δ} {v m₁ m₂ B₁ B₂}
   (hcase : Γ ∣ ⬝ ⊢ case v m₁ m₂ ∶ Prod B₁ B₂) :
   Γ ∣ Δ ⊨ snd (case v m₁ m₂) ~ case v (snd m₁) (snd m₂) ∶ B₂ := by
   intro σ τ hστ js₁ js₂ hjs
   let ⟨_, n₁, _, n₂, r₁, r₂, hB₁⟩ := (soundCom hcase hστ .nil).snd
-  have r₁' : snd ((case v m₁ m₂)⦃σ⦄) ⇒⋆ n₁ := .trans' r₁.snd (.once .π2)
+  have r₁' : snd ((case v m₁ m₂)⦃σ⦄) ⇒⋆ n₁ := by
+    rw [← @weakenJCom0 n₁]; exact .trans' r₁.snd (.once .π2)
   simp only [substCom] at *
   cases hcase with | case hv hm₁ hm₂ =>
   let hv := soundVal hv hστ; unfold 𝒱 at hv
@@ -259,55 +272,47 @@ theorem sndCase {Γ Δ v m₁ m₂ B₁ B₂}
     let ⟨_, _, _, _, _, r₂', _⟩ := (soundCom hm₁ (semCtxt.cons hA₁ hστ) .nil).snd
     let ⟨_, rprod₁, r'⟩ := confluence r₂ (.once .ιl); rw [substUnion] at r'
     let ⟨_, rprod₂, r'⟩ := confluence r₂' r'; rw [← rprod₂.prod_inv] at r'
-    injection Evals.prod_inv (.trans' rprod₁ r') with en₁ en₂; subst en₁ en₂
+    injection Evals.prod_inv (.trans' rprod₁ r') with _ en₁ en₂; subst en₁ en₂
     clear rprod₁ rprod₂ r' r₁; clear r'
     have r₂' :
       case (inl v₂) (snd (m₁⦃⇑ τ⦄)) (snd (m₂⦃⇑ τ⦄)) ⇒⋆ n₂ := calc
       _ ⇒  snd (m₁⦃⇑ τ⦄)⦃v₂⦄ := .ιl
       _ =  snd (m₁⦃v₂ +: τ⦄) := by simp only [substCom]; rw [substUnion]
       _ ⇒⋆ snd (prod _ n₂)   := r₂'.snd
-      _ ⇒ n₂                 := .π2
+      _ ⇒  weakenJCom 0 n₂   := .π2
+      _ ⇒⋆ n₂                := by rw [weakenJCom0]
     exact ℰ.bwdsRejoin r₁' r₂' hB₁
   | .inr ⟨v₁, v₂, hA₂, e₁, e₂⟩ =>
     rw [e₂]; rw [e₂] at r₂
     let ⟨_, _, _, _, _, r₂', _⟩ := (soundCom hm₂ (semCtxt.cons hA₂ hστ) .nil).snd
     let ⟨_, rprod₁, r'⟩ := confluence r₂ (.once .ιr); rw [substUnion] at r'
     let ⟨_, rprod₂, r'⟩ := confluence r₂' r'; rw [← rprod₂.prod_inv] at r'
-    injection Evals.prod_inv (.trans' rprod₁ r') with en₁ en₂; subst en₁ en₂
+    injection Evals.prod_inv (.trans' rprod₁ r') with _ en₁ en₂; subst en₁ en₂
     clear rprod₁ rprod₂ r' r₁; clear r'
     have r₂' :
       case (inr v₂) (snd (m₁⦃⇑ τ⦄)) (snd (m₂⦃⇑ τ⦄)) ⇒⋆ n₂ := calc
       _ ⇒  snd (m₂⦃⇑ τ⦄)⦃v₂⦄ := .ιr
       _ =  snd (m₂⦃v₂ +: τ⦄) := by simp only [substCom]; rw [substUnion]
       _ ⇒⋆ snd (prod _ n₂)   := r₂'.snd
-      _ ⇒ n₂                 := .π2
+      _ ⇒  weakenJCom 0 n₂   := .π2
+      _ ⇒⋆ n₂                := by rw [weakenJCom0]
     exact ℰ.bwdsRejoin r₁' r₂' hB₁
 
-theorem joinJoin {Γ Δ n₁ n₂ m A B} (hn₁ : Γ ∷ A ∣ Δ ⊢ n₁ ∶ B) (hn₂ : Γ ∷ A ∣ Δ ∷ A ↗ B ⊢ n₂ ∶ B) (hm : Γ ∣ Δ ∷ A ↗ B ⊢ m ∶ B) :
-  Γ ∣ Δ ⊨ join (join (renameCom (lift succ) n₁) n₂) m ~ join n₁ (join n₂ (renameJCom (lift succ) m)) ∶ B := by
+theorem joinJoin {Γ δ} {Δ : Dtxt δ} {n₁ n₂ m A B} (hn₁ : Γ ∷ A ∣ Δ ⊢ n₁ ∶ B) (hn₂ : Γ ∷ A ∣ Δ ∷ A ↗ B ⊢ n₂ ∶ B) (hm : Γ ∣ Δ ∷ A ↗ B ⊢ m ∶ B) :
+  Γ ∣ Δ ⊨ join (join (renameCom (lift succ) n₁) n₂) m ~ join n₁ (join n₂ (renameJCom (liftJ Fin.succ) m)) ∶ B := by
   intro σ τ hστ js₁ js₂ hjs
-  have hn := ComWt.join (wtWeakenCom₂ hn₁) hn₂
-  refine ℰ.bwdsRejoin .refl .refl ?_
-  have hjsn₁' := semDtxt.cons hjs (λ hvw ↦
-    have hn := soundCom hn₁ (semCtxt.cons hvw hστ) hjs
-    by rw [← substUnion σ, ← substUnion τ] at hn; exact hn)
-  have hjsn₁ := semDtxt.cons hjs (λ hvw ↦
-    have hn := soundCom hn (semCtxt.cons hvw hστ) hjs
-    by rw [substUnion σ, substUnion τ]; exact hn)
-  have what := soundCom hm hστ hjsn₁; simp only [rejoin] at what
   sorry
 
-theorem dropJoin {Γ Δ m₁ m₂ A B} (h₁ : Γ ∷ A ∣ Δ ⊢ m₁ ∶ B) (h₂ : Γ ∣ Δ ⊢ m₂ ∶ B) :
-  ∀ σ τ, Γ ⊨ σ ~ τ → ∀ js₁ js₂, Δ ⊨ js₁ ~ js₂ → ScopeSubstJ τ →
-  (rejoin (m₂⦃σ⦄) js₁, rejoin ((join m₁ (renameJCom succ m₂))⦃τ⦄) js₂) ∈ ⟦B⟧ᵉ := by
-  intro σ τ hστ js₁ js₂ hjs hτ
+theorem dropJoin {Γ δ} {Δ : Dtxt δ} {m₁ m₂ A B} (h₁ : Γ ∷ A ∣ Δ ⊢ m₁ ∶ B) (h₂ : Γ ∣ Δ ⊢ m₂ ∶ B) :
+  Γ ∣ Δ ⊨ m₂ ~ (join m₁ (renameJCom Fin.succ m₂)) ∶ B := by
+  intro σ τ hστ js₁ js₂ hjs
   -- get rid of join m₁
   have hm₂ := soundCom (.join h₁ (wtWeakenJ h₂)) hστ hjs
   unfold ℰ at hm₂
   let ⟨_, n₂, _, rn₂, _⟩ := hm₂
   have nfn₂ := rn₂.2
   simp [renameJSubst] at rn₂; simp [renameJSubst]
-  let ⟨_, rm₂, rjoin, rn₂⟩ := rn₂.wkJoin (h₂.scopeJ.subst hτ)
+  let ⟨_, rm₂, rjoin, rn₂⟩ := rn₂.wkJoin
   refine ℰ.bwds .refl (.trans' rjoin rn₂) ?_
   -- merge reductions via confluence
   have hm₂ := soundCom h₂ hστ hjs
@@ -317,7 +322,7 @@ theorem dropJoin {Γ Δ m₁ m₂ A B} (h₁ : Γ ∷ A ∣ Δ ⊢ m₁ ∶ B) (
   rw [nfn₂'.steps rn'] at hB' nfn₂'
   unfold ℰ; exact ⟨_, _, rn₁, ⟨rn, nfn₂'⟩, hB'⟩
 
-theorem caseOfCase {Γ Δ v m₁ m₂ m₃ m₄ B} {A₁ A₂ A₃ A₄ : ValType}
+theorem caseOfCase {Γ δ} {Δ : Dtxt δ} {v m₁ m₂ m₃ m₄ B} {A₁ A₂ A₃ A₄ : ValType}
   (hv : Γ ⊢ v ∶ Sum A₃ A₄)
   (hm₁ : Γ ∷ A₁ ∣ Δ ⊢ m₁ ∶ B)
   (hm₂ : Γ ∷ A₂ ∣ Δ ⊢ m₂ ∶ B)
@@ -325,7 +330,7 @@ theorem caseOfCase {Γ Δ v m₁ m₂ m₃ m₄ B} {A₁ A₂ A₃ A₄ : ValTyp
   (hm₄ : Γ ∷ A₄ ∣ ⬝ ⊢ m₄ ∶ F (Sum A₁ A₂)) :
   Γ ∣ Δ ⊨ join (case (var 0) (renameCom (lift succ) m₁) (renameCom (lift succ) m₂))
             (case v (letin m₃ (jump 0 (var 0))) (letin m₄ (jump 0 (var 0))))
-        ~ join m₁ (join (renameJCom succ m₂)
+        ~ join m₁ (join (renameJCom Fin.succ m₂)
             (case v (letin m₃ (case (var 0) (jump 1 (var 0)) (jump 0 (var 0))))
                     (letin m₄ (case (var 0) (jump 1 (var 0)) (jump 0 (var 0)))))) ∶ B := by
   intro σ τ hστ js₁ js₂ hjs
@@ -345,7 +350,7 @@ theorem caseOfCase {Γ Δ v m₁ m₂ m₃ m₄ B} {A₁ A₂ A₃ A₄ : ValTyp
       subst e₁ e₂
       refine ℰ.bwds
         (.rejoin (.trans .γ (.once .ιl)))
-        (.rejoin (.trans' (Evals.join (.trans (.join .ιl) (.once .join't))) (.once .γ))) ?_
+        (.rejoin (.trans' (Evals.join (.trans (.join .ιl) (.once (.join't (j := 0))))) (.once .γ))) ?_
       rw [substUnion, substUnion, substUnion₂, substDrop₂]; simp [up]
       exact soundCom hm₁ (semCtxt.cons hA₁ hστ) hjs
     | .inr ⟨w₁', w₂', hA₂, e₁, e₂⟩ =>
@@ -354,8 +359,8 @@ theorem caseOfCase {Γ Δ v m₁ m₂ m₃ m₄ B} {A₁ A₂ A₃ A₄ : ValTyp
         (.rejoin (.trans .γ (.once .ιr)))
         (.rejoin (.join (.trans (.join .ιr) (.once .γ)))) ?_
       rw [substUnion, substUnion, substUnion₂, substDrop₂]; simp [up]
-      have hB := soundCom hm₂ (semCtxt.cons hA₂ hστ) hjs
-      sorry
+      have hB := dropJoin (wtWeakenCom₂ hm₁) hm₂ (semCtxt.cons hA₂ hστ) hjs
+      simp [renameUpSubstCons] at hB; exact hB
   | .inr ⟨v₁, v₂, hA₄, e₁, e₂⟩ =>
     simp only [substCom]; rw [e₁, e₂]
     refine ℰ.bwd (.rejoin (.join .ιr)) (.rejoin (.join (.join .ιr))) ?_
@@ -370,7 +375,7 @@ theorem caseOfCase {Γ Δ v m₁ m₂ m₃ m₄ B} {A₁ A₂ A₃ A₄ : ValTyp
       subst e₁ e₂
       refine ℰ.bwds
         (.rejoin (.trans .γ (.once .ιl)))
-        (.rejoin (.trans' (Evals.join (.trans (.join .ιl) (.once .join't))) (.once .γ))) ?_
+        (.rejoin (.trans' (Evals.join (.trans (.join .ιl) (.once (.join't (j := 0))))) (.once .γ))) ?_
       rw [substUnion, substUnion, substUnion₂, substDrop₂]; simp [up]
       exact soundCom hm₁ (semCtxt.cons hA₁ hστ) hjs
     | .inr ⟨w₁', w₂', hA₂, e₁, e₂⟩ =>
@@ -379,5 +384,5 @@ theorem caseOfCase {Γ Δ v m₁ m₂ m₃ m₄ B} {A₁ A₂ A₃ A₄ : ValTyp
         (.rejoin (.trans .γ (.once .ιr)))
         (.rejoin (.join (.trans (.join .ιr) (.once .γ)))) ?_
       rw [substUnion, substUnion, substUnion₂, substDrop₂]; simp [up]
-      have hB := soundCom hm₂ (semCtxt.cons hA₂ hστ) hjs
-      sorry
+      have hB := dropJoin (wtWeakenCom₂ hm₁) hm₂ (semCtxt.cons hA₂ hστ) hjs
+      simp [renameUpSubstCons] at hB; exact hB
