CBPV/Typing.lean
@@ -27,7 +27,7 @@ inductive ValWt : Ctxt → Val → ValType → Prop where
     -----------------
     Γ ⊢ thunk m ∶ U B
 
-inductive ComWt : Ctxt → Dtxt → Com → ComType → Prop where
+inductive ComWt : ∀ {δ}, Ctxt → Dtxt δ → Com δ → ComType → Prop where
   | force {Γ Δ v B} :
     Γ ⊢ v ∶ U B →
     -------------------
@@ -91,7 +91,7 @@ notation:40 Γ:41 "∣" Δ:41 "⊢" m:41 "∶" B:41 => ComWt Γ Δ m B
 
 theorem wtRename {ξ} {Γ Ξ : Ctxt} (hξ : Ξ ⊢ ξ ∶ Γ) :
   (∀ {v} {A : ValType}, Γ ⊢ v ∶ A → Ξ ⊢ renameVal ξ v ∶ A) ∧
-  (∀ {Δ m} {B : ComType}, Γ ∣ Δ ⊢ m ∶ B → Ξ ∣ Δ ⊢ renameCom ξ m ∶ B) := by
+  (∀ {δ} {Δ : Dtxt δ} {m : Com δ} {B : ComType}, Γ ∣ Δ ⊢ m ∶ B → Ξ ∣ Δ ⊢ renameCom ξ m ∶ B) := by
   refine ⟨λ h ↦ ?wtv, λ h ↦ ?wtm⟩
   mutual_induction h, h generalizing ξ Ξ
   all_goals constructor <;> apply_rules [wRenameLift]
@@ -100,7 +100,7 @@ theorem wtRenameVal {ξ} {Γ Δ : Ctxt} {v} {A : ValType} :
   Δ ⊢ ξ ∶ Γ → Γ ⊢ v ∶ A → Δ ⊢ renameVal ξ v ∶ A :=
   λ hξ ↦ (wtRename hξ).left
 
-theorem wtRenameCom {ξ} {Γ Ξ : Ctxt} {Δ m} {B : ComType} :
+theorem wtRenameCom {ξ} {Γ Ξ : Ctxt} {δ} {Δ : Dtxt δ} {m : Com δ} {B : ComType} :
   Ξ ⊢ ξ ∶ Γ → Γ ∣ Δ ⊢ m ∶ B → Ξ ∣ Δ ⊢ renameCom ξ m ∶ B :=
   λ hξ ↦ (wtRename hξ).right
 
@@ -108,55 +108,55 @@ theorem wtWeakenVal {Γ A₁ A₂} {v : Val} :
   Γ ⊢ v ∶ A₂ → Γ ∷ A₁ ⊢ renameVal succ v ∶ A₂ :=
     wtRenameVal wRenameSucc
 
-theorem wtWeakenCom {Γ Δ A B} {m : Com} :
+theorem wtWeakenCom {Γ δ Δ A B} {m : Com δ} :
   Γ ∣ Δ ⊢ m ∶ B → Γ ∷ A ∣ Δ ⊢ renameCom succ m ∶ B :=
   wtRenameCom wRenameSucc
 
-theorem wtWeakenCom₂ {Γ Δ A₁ A₂ B} {m : Com} :
+theorem wtWeakenCom₂ {Γ δ Δ A₁ A₂ B} {m : Com δ} :
   Γ ∷ A₂ ∣ Δ ⊢ m ∶ B → Γ ∷ A₁ ∷ A₂ ∣ Δ ⊢ renameCom (lift succ) m ∶ B :=
   wtRenameCom (wRenameLift wRenameSucc)
 
 /-* Jump renaming and weakening *-/
 
-theorem wtRenameJ {ξ Γ} {Δ Φ : Dtxt} {m B} (hξ : Φ ⊢ ξ ∶ Δ)
+theorem wtRenameJ {Γ} {δ δ' ξ} {Δ : Dtxt δ} {Φ : Dtxt δ'} {m B} (hξ : Φ ⊢ ξ ∶ Δ)
   (h : Γ ∣ Δ ⊢ m ∶ B) : Γ ∣ Φ ⊢ renameJCom ξ m ∶ B := by
-  mutual_induction h generalizing ξ Φ
+  mutual_induction h generalizing ξ δ' Φ
   all_goals constructor <;> apply_rules [wRenameJLift]
 
-theorem wtWeakenJ {Γ Δ A' B' B} {m : Com} :
-  Γ ∣ Δ ⊢ m ∶ B → Γ ∣ Δ ∷ A' ↗ B' ⊢ renameJCom succ m ∶ B :=
+theorem wtWeakenJ {Γ δ Δ A' B' B} {m : Com δ} :
+  Γ ∣ Δ ⊢ m ∶ B → Γ ∣ Δ ∷ A' ↗ B' ⊢ renameJCom Fin.succ m ∶ B :=
   wtRenameJ wRenameJSucc
 
 /-*--------------------------------------
   Rearrangement lemmas for commutations
 --------------------------------------*-/
 
-theorem wtLetApp {Γ Δ n m v A B} (hlet : Γ ∣ ⬝ ⊢ letin n m ∶ Arr A B) (hv : Γ ⊢ v ∶ A) :
+theorem wtLetApp {Γ δ} {Δ : Dtxt δ} {n m v A B} (hlet : Γ ∣ ⬝ ⊢ letin n m ∶ Arr A B) (hv : Γ ⊢ v ∶ A) :
   Γ ∣ Δ ⊢ letin n (app m (renameVal succ v)) ∶ B := by
   cases hlet with | letin hn hm =>
   exact .letin hn (.app hm (wtWeakenVal hv))
 
-theorem wtLetFst {Γ Δ n m B₁ B₂} (hlet : Γ ∣ ⬝ ⊢ letin n m ∶ Prod B₁ B₂) :
+theorem wtLetFst {Γ δ} {Δ : Dtxt δ} {n m B₁ B₂} (hlet : Γ ∣ ⬝ ⊢ letin n m ∶ Prod B₁ B₂) :
   Γ ∣ Δ ⊢ letin n (fst m) ∶ B₁ := by
   cases hlet with | letin hn hm =>
   exact .letin hn (.fst hm)
 
-theorem wtLetSnd {Γ Δ n m B₁ B₂} (hlet : Γ ∣ ⬝ ⊢ letin n m ∶ Prod B₁ B₂) :
+theorem wtLetSnd {Γ δ} {Δ : Dtxt δ} {n m B₁ B₂} (hlet : Γ ∣ ⬝ ⊢ letin n m ∶ Prod B₁ B₂) :
   Γ ∣ Δ ⊢ letin n (snd m) ∶ B₂ := by
   cases hlet with | letin hn hm =>
   exact .letin hn (.snd hm)
 
-theorem wtCaseApp {Γ Δ v m₁ m₂ w A B} (hcase : Γ ∣ ⬝ ⊢ case v m₁ m₂ ∶ Arr A B) (hw : Γ ⊢ w ∶ A) :
+theorem wtCaseApp {Γ δ} {Δ : Dtxt δ} {v m₁ m₂ w A B} (hcase : Γ ∣ ⬝ ⊢ case v m₁ m₂ ∶ Arr A B) (hw : Γ ⊢ w ∶ A) :
   Γ ∣ Δ ⊢ case v (app m₁ (renameVal succ w)) (app m₂ (renameVal succ w)) ∶ B := by
   cases hcase with | case hv hm₁ hm₂ =>
   exact .case hv (.app hm₁ (wtWeakenVal hw)) (.app hm₂ (wtWeakenVal hw))
 
-theorem wtCaseFst {Γ Δ v m₁ m₂ B₁ B₂} (hcase : Γ ∣ ⬝ ⊢ case v m₁ m₂ ∶ Prod B₁ B₂) :
+theorem wtCaseFst {Γ δ} {Δ : Dtxt δ} {v m₁ m₂ B₁ B₂} (hcase : Γ ∣ ⬝ ⊢ case v m₁ m₂ ∶ Prod B₁ B₂) :
   Γ ∣ Δ ⊢ case v (fst m₁) (fst m₂) ∶ B₁ := by
   cases hcase with | case hv hm₁ hm₂ =>
   exact .case hv (.fst hm₁) (.fst hm₂)
 
-theorem wtCaseSnd {Γ Δ v m₁ m₂ B₁ B₂} (hcase : Γ ∣ ⬝ ⊢ case v m₁ m₂ ∶ Prod B₁ B₂) :
+theorem wtCaseSnd {Γ δ} {Δ : Dtxt δ} {v m₁ m₂ B₁ B₂} (hcase : Γ ∣ ⬝ ⊢ case v m₁ m₂ ∶ Prod B₁ B₂) :
   Γ ∣ Δ ⊢ case v (snd m₁) (snd m₂) ∶ B₂ := by
   cases hcase with | case hv hm₁ hm₂ =>
   exact .case hv (.snd hm₁) (.snd hm₂)
